# 2017 AMC 12A Problem 23

## Problem

For certain real numbers $a$ , $b$ , and $c$ , the polynomial \[g(x) = x^3 + ax^2 + x + 10\] has three distinct roots, and each root of $g(x)$ is also a root of the polynomial \[f(x) = x^4 + x^3 + bx^2 + 100x + c.\] What is $f(1)$ ?

$\textbf{(A)}\ -9009 \qquad\textbf{(B)}\ -8008 \qquad\textbf{(C)}\ -7007 \qquad\textbf{(D)}\ -6006 \qquad\textbf{(E)}\ -5005$

## Solution
Let $r_1,r_2,$ and $r_3$ be the roots of $g(x)$ . Let $r_4$ be the additional root of $f(x)$ . Then from Vieta's formulas on the quadratic term of $g(x)$ and the cubic term of $f(x)$ , we obtain the following:
\begin{align*} r_1+r_2+r_3&=-a \\ r_1+r_2+r_3+r_4&=-1 \end{align*}
Thus $r_4=a-1$ .
Now applying Vieta's formulas on the constant term of $g(x)$ , the linear term of $g(x)$ , and the linear term of $f(x)$ , we obtain:
\begin{align*} r_1r_2r_3 & = -10\\ r_1r_2+r_2r_3+r_3r_1 &= 1\\ r_1r_2r_3+r_2r_3r_4+r_3r_4r_1+r_4r_1r_2 & = -100\\ \end{align*}
Substituting for $r_1r_2r_3$ in the bottom equation and factoring the remainder of the expression, we obtain:
\[-10+(r_1r_2+r_2r_3+r_3r_1)r_4=-10+r_4=-100\]
It follows that $r_4=-90$ . But $r_4=a-1$ so $a=-89$
Now we can factor $f(x)$ in terms of $g(x)$ as
\[f(x)=(x-r_4)g(x)=(x+90)g(x)\]
Then $f(1)=91g(1)$ and
\[g(1)=1^3-89\cdot 1^2+1+10=-77\]
Hence $f(1)=91\cdot(-77)=\boxed{\textbf{(C)}\,-7007}$ .

## Solution 2
Since all of the roots of $g(x)$ are distinct and are roots of $f(x)$ , and the degree of $f$ is one more than the degree of $g$ , we have that
\[f(x) = C(x-k)g(x)\]
for some number $k$ . By comparing $x^4$ coefficients, we see that $C=1$ . Thus,
\[x^4+x^3+bx^2+100x+c=(x-k)(x^3+ax^2+x+10)\]
Expanding and equating coefficients we get that
\[a-k=1,1-ak=b,10-k=100,-10k=c\]
The third equation yields $k=-90$ , and the first equation yields $a=-89$ . So we have that
$f(1)=(1+90)g(1)=91(1-89+1+10)=(91)(-77)=\boxed{\textbf{(C)}\,-7007}$

## Solution 3
Let the roots of $g(x)$ be $p,q,r$ and the roots of $f(x)$ be $p,q,r,s$ . Then by Vietas, \[-100=pqr+pqs+prs+qrs = -10+ s(pq+pr+rs) = -10 + s,\] so $s = -90$ . Again by Vietas, $p+q+r+s = -a + s = -1 \implies a = -89$ . Finally, $f(1) = (1-(-90))g(1) = \textbf{(C)}\,-7007$ .

## Solution 4
$f(x)$ must have four roots, three of which are roots of $g(x)$ . Using the fact that every polynomial has a unique factorization into its roots, and since the leading coefficient of $f(x)$ and $g(x)$ are the same, we know that
\[f(x)=g(x)(x-r)\]
where $r\in\mathbb{C}$ is the fourth root of $f(x)$ . Substituting $g(x)$ and expanding, we find that
\begin{align*}f(x)&=(x^3+ax^2+x+10)(x-r)\\ &=x^4+(a-r)x^3+(1-ar)x^2+(10-r)x-10r.\end{align*}
Comparing coefficients with $f(x)$ , we see that
\begin{align*} a-r&=1\\ 1-ar&=b\\ 10-r&=100\\ -10r&=c.\\ \end{align*}
(Solution 1.1 picks up here.)
Let's solve for $a,b,c,$ and $r$ . Since $10-r=100$ , $r=-90$ , so $c=(-10)(-90)=900$ . Since $a-r=1$ , $a=-89$ , and $b=1-ar=-8009$ . Thus, we know that
\[f(x)=x^4+x^3-8009x^2+100x+900.\]
Taking $f(1)$ , we find that
\begin{align*} f(1)&=1^4+1^3-8009(1)^2+100(1)+900\\ &=1+1-8009+100+900\\ &=\boxed{\bold{(C)}\, -7007}.\\ \end{align*}

## Solution 5
A faster ending to Solution 1 is as follows. We shall solve for only $a$ and $r$ . Since $10-r=100$ , $r=-90$ , and since $a-r=1$ , $a=-89$ . Then, \begin{align*} f(1)&=(1-r)(1^3+a\cdot1^2+1+10)\\ &=(91)(-77)\\ &=\boxed{\bold{(C)}\, -7007}.\\ \end{align*}

## Solution 6 (Fast)
Let the term $q(x)$ be the linear term that we are solving for in the equation $f(x)=g(x)\cdot q(x)$ . Now, we know that $q(x)=mx-r$ must have $m=1$ , because only $x \cdot x^3=x^4$ . In addition, we know that, by distributing, $10x-rx=100x$ . Therefore, $r=-90$ , and all the other variables are quickly solved for.

## Solution 7
We notice that the constant term of $f(x)=c$ and the constant term in $g(x)=10$ . Because $f(x)$ can be factored as $g(x) \cdot (x- r)$ (where $r$ is the unshared root of $f(x)$ , we see that using the constant term, $-10 \cdot r = c$ and therefore $r = -\frac{c}{10}$ . Now we once again write $f(x)$ out in factored form:
\[f(x) = g(x)\cdot (x-r) = (x^3+ax^2+x+10)\left(x+\frac{c}{10}\right)\] .
We can expand the expression on the right-hand side to get:
\[f(x) = x^4+\left(a+\frac{c}{10}\right)x^3+\left(1+\frac{ac}{10}\right)x^2+\left(10+\frac{c}{10}\right)x+c\]
Now we have $f(x) = x^4+\left(a+\frac{c}{10}\right)x^3+\left(1+\frac{ac}{10}\right)x^2+\left(10+\frac{c}{10} \right)x+c=x^4+x^3+bx^2+100x+c$ .
Simply looking at the coefficients for each corresponding term (knowing that they must be equal), we have the equations: \[10+\frac{c}{10}=100 \Rightarrow c=900\] \[a+\frac{c}{10} = 1, c=900 \Rightarrow a + 90 =1 \Rightarrow a= -89\]
and finally,
\[1+\frac{ac}{10} = b = 1+\frac{-89 \cdot 900}{10} = b = -8009\] .
We know that $f(1)$ is the sum of its coefficients, hence $1+1+b+100+c$ . We substitute the values we obtained for $b$ and $c$ into this expression to get $f(1) = 1 + 1 + (-8009) + 100 + 900 = \boxed{\textbf{(C)}\,-7007}$ .

## Solution 8
Let $r_1,r_2,$ and $r_3$ be the roots of $g(x)$ . Let $r_4$ be the additional root of $f(x)$ . Then from Vieta's formulas on the quadratic term of $g(x)$ and the cubic term of $f(x)$ , we obtain the following:
\begin{align*} r_1+r_2+r_3&=-a \\ r_1+r_2+r_3+r_4&=-1 \end{align*}
Thus $r_4=a-1$ .
Now applying Vieta's formulas on the constant term of $g(x)$ , the linear term of $g(x)$ , and the linear term of $f(x)$ , we obtain:
\begin{align*} r_1r_2r_3 & = -10\\ r_1r_2+r_2r_3+r_3r_1 &= 1\\ r_1r_2r_3+r_2r_3r_4+r_3r_4r_1+r_4r_1r_2 & = -100\\ \end{align*}
Substituting for $r_1r_2r_3$ in the bottom equation and factoring the remainder of the expression, we obtain:
\[-10+(r_1r_2+r_2r_3+r_3r_1)r_4=-10+r_4=-100\]
It follows that $r_4=-90$ . But $r_4=a-1$ so $a=-89$
Now we can factor $f(x)$ in terms of $g(x)$ as
\[f(x)=(x-r_4)g(x)=(x+90)g(x)\]
Then $f(1)=91g(1)$ and
\[g(1)=1^3-89\cdot 1^2+1+10=-77\]
Hence $f(1)=91\cdot(-77)=\boxed{\textbf{(C)}\,-7007}$ .

## Solution 9 (Risky)
Let the roots of $g(x)$ be $r_1$ , $r_2$ , and $r_3$ . Let the roots of $f(x)$ be $r_1$ , $r_2$ , $r_3$ , and $r_4$ . From Vieta's, we have: \begin{align*} r_1+r_2+r_3=-a \\ r_1+r_2+r_3+r_4=-1 \\ r_4=a-1 \end{align*} The fourth root is $a-1$ . Since $r_1$ , $r_2$ , and $r_3$ are common roots, we have: \begin{align*} f(x)=g(x)(x-(a-1)) \\ f(1)=g(1)(1-(a-1)) \\ f(1)=(a+12)(2-a) \\ f(1)=-(a+12)(a-2) \\ \end{align*} Let $a-2=k$ : \begin{align*} f(1)=-k(k+14) \end{align*} Note that $-7007=-1001\cdot(7)=-(7\cdot(11)\cdot(13))\cdot(7)=-91\cdot(77)$ This gives us a pretty good guess of $\boxed{\textbf{(C)}\, -7007}$ .

## Solution 10
First off, let's get rid of the $x^4$ term by finding $h(x)=f(x)-xg(x)$ . This polynomial consists of the difference of two polynomials with $3$ common factors, so it must also have these factors. The polynomial is $h(x)=(1-a)x^3 + (b-1)x^2 + 90x + c$ , and must be equal to $(1-a)g(x)$ . Equating the coefficients, we get $3$ equations. We will tackle the situation one equation at a time, starting the $x$ terms. Looking at the coefficients, we get $\dfrac{90}{1-a} = 1$ . \[\therefore 90=1-a.\] The solution to the previous is obviously $a=-89$ . We can now find $b$ and $c$ . $\dfrac{b-1}{1-a} = a$ , \[\therefore b-1=a(1-a)=-89\cdot90=-8010\] and $b=-8009$ . Finally $\dfrac{c}{1-a} = 10$ , \[\therefore c=10(1-a)=10\cdot90=900\] Solving the original problem, $f(1)=1 + 1 + b + 100 + c = 102+b+c=102+900-8009=\boxed{\textbf{©}\, -7007}$ .

## Solution 11
Simple polynomial division is a feasible method. Even though we have variables, we can equate terms at the end of the division so that we can cancel terms. Doing the division of $\frac{f(x)}{g(x)}$ eventually brings us the final step $(1-a)x^3 + (b-1)x^2 + 90x + c$ minus $(1-a)x^3 - (a-a^2)x^2 + (1-a)x + 10(1-a)$ after we multiply $f(x)$ by $(1-a)$ . Now we equate coefficients of same-degree $x$ terms. This gives us $10(1-a) = c, b-1 = a - a^2, 1-a = 90 \Rightarrow a = -89, c = 900, b = -8009$ . We are interested in finding $f(1)$ , which equals $1^4 + 1^3 -8009\cdot1^2 + 100\cdot1 + 900 = \boxed{\textbf{(C)}\,-7007}$ . ~skyscraper
### Note
Note that $f(1)$ for any polynomial is simply the sum of the coefficients of the polynomial.

## Video Solution 1
https://youtu.be/MBIiz0mroqk

## Video Solution 2
https://youtu.be/3dfbWzOfJAI?t=4412 ~ pi_is_3.14

## Video Solution 3 by Punxsutawney Phil
https://youtu.be/i1GpjPXtrPA
### See Also
These problems are copyrighted © by the Mathematical Association of America.
These problems are copyrighted © by the Mathematical Association of America.
These problems are copyrighted © by the Mathematical Association of America.
These problems are copyrighted © by the Mathematical Association of America .