# 2016 AMC 12B Problem 21

## Problem

Let $ABCD$ be a unit square. Let $Q_1$ be the midpoint of $\overline{CD}$ . For $i=1,2,\dots,$ let $P_i$ be the intersection of $\overline{AQ_i}$ and $\overline{BD}$ , and let $Q_{i+1}$ be the foot of the perpendicular from $P_i$ to $\overline{CD}$ . What is \[\sum_{i=1}^{\infty} \text{Area of } \triangle DQ_i P_i \, ?\]

$\textbf{(A)}\ \frac{1}{6} \qquad \textbf{(B)}\ \frac{1}{4} \qquad \textbf{(C)}\ \frac{1}{3} \qquad \textbf{(D)}\ \frac{1}{2} \qquad \textbf{(E)}\ 1$

## Solutions

## Solution 1
We start with $DQ_i = 1/2$ for $i = 1.$ $\triangle BP_iA \sim \triangle DP_iQ_i$ and $\triangle DP_iQ_{i+1} \sim \triangle DBC$ so we have \[\frac{DQ_i}{AB} = \frac{DP_i}{P_iB} = \frac{1}{2} \implies \frac{DP_i}{BD} = \frac{DQ_{i+1}}{DC} = \frac{DQ_{i+1}}{1} = \frac{1}{3} \implies DQ_{i+1} = DQ_{2} = \frac{1}{3}.\] Repeating this same process for subsequent $i$ s yields $DQ_3 = \frac{1}{4}, DQ_4 = \frac{1}{5}, DQ_5 = \frac{1}{6} \dots$ We can generalize this by saying $DQ_i = \frac{1}{i + 1}.$ Then $[ADQ_i] = \frac{1}{2(i + 1)}.$ Let $y = [AP_iD]$ and let $x = [DP_iQ_i].$ $\triangle BP_iA$ and $\triangle DP_iQ_i$ are similar with side length ratio $(i + 1):1$ , so $[BP_iA] = (i + 1)^2x.$ Now, we can express the area of $\triangle ADB$ (which is $1/2$ since it's just half the square) as $y + (i + 1)^2x,$ and we can express the area of $ADQ_i$ as $x + y.$ We have a system of equations:
\[[ADQ_i] = x + y = \frac{1}{2(i + 1)}\] \[[ADB] = (i + 1)^2x + y = \frac{1}{2}.\]
Solving, we get $x = \frac{1}{2(i+1)(i+2)}.$ So now the problem becomes $\sum_{i=1}^{\infty} \frac{1}{2(i+1)(i+2)}$ . We can rewrite this as \[\frac{1}{2} \sum_{i=1}^{\infty} \left( \frac{1}{i+1} - \frac{1}{i+2} \right) = \frac{1}{2} \left( \left( \frac{1}{2} - \frac{1}{3} \right) + \left( \frac{1}{3} - \frac{1}{4} \right) + \left( \frac{1}{4} - \frac{1}{5} \right) + \dots \right)\]
All terms cancel except for the $\frac{1}{2}$ on the inside and $\frac{1}{2}$ on the outside, so the answer is $\boxed{\frac{1}{4}}.$
~ grogg007

## Solution 2
(By Qwertazertl)
We are tasked with finding the sum of the areas of every $\triangle DQ_i^{}P_i^{}$ where $i$ is a positive integer. We can start by finding the area of the first triangle, $\triangle DQ_1^{}P_1^{}$ . This is equal to $\frac{1}{2}$ ⋅ $DQ_1^{}$ ⋅ $P_1^{}Q_2^{}$ . Notice that since triangle $\triangle DQ_1^{}P_1^{}$ is similar to triangle $\triangle ABP_1^{}$ in a 1 : 2 ratio, $P_1^{}Q_2^{}$ must equal $\frac{1}{3}$ (since we are dealing with a unit square whose side lengths are 1). $DQ_1^{}$ is of course equal to $\frac{1}{2}$ as it is the mid-point of CD. Thus, the area of the first triangle is $[DQ_1P_1]=\frac{1}{2}$ ⋅ $\frac{1}{2}$ ⋅ $\frac{1}{3}$ .
The second triangle has a base $DQ_2^{}$ equal to that of $P_1^{}Q_2^{}$ (see that $\triangle DQ_2^{}P_1^{}$ ~ $\triangle DCB$ ) and using the same similar triangle logic as with the first triangle, we find the area to be $[DQ_2P_2]=\frac{1}{2}$ ⋅ $\frac{1}{3}$ ⋅ $\frac{1}{4}$ . If we continue and test the next few triangles, we will find that the sum of all $\triangle DQ_i^{}P_i^{}$ is equal to \[\frac{1}{2} \sum\limits_{n=2}^\infty \frac{1}{n(n+1)}\] or \[\frac{1}{2} \sum\limits_{n=2}^\infty \left(\frac{1}{n} - \frac{1}{n+1}\right)\]
This is known as a telescoping series because we can see that every term after the first $\frac{1}{n}$ is going to cancel out. Thus, the summation is equal to $\frac{1}{2}$ and after multiplying by the half out in front, we find that the answer is $\boxed{\textbf{(B) }\frac{1}{4}}$ .

## Solution 3
(By mastermind.hk16)
Note that $AD \|\ P_iQ_{i+1}\ \forall i \in \mathbb{N}$ . So $\triangle ADQ_i \sim \triangle P_{i}Q_{i+1}Q_{i} \ \forall i \in \mathbb{N}$
Hence $\frac{Q_iQ_{i+1}}{DQ_{i}}=\frac{P_{i}Q_{i+1}}{AD} \ \ \Longrightarrow DQ_i \cdot P_iQ_{i+1}=Q_iQ_{i+1}$
We compute $\frac{1}{2} \sum_{i=1}^{\infty}DQ_i \cdot P_iQ_{i+1}= \frac{1}{2} \sum_{i=1}^{\infty}Q_iQ_{i+1}=\frac{1}{2} \cdot DQ_1 =\frac{1}{4}$ because $Q_i \rightarrow D$ as $i \rightarrow \infty$ .

## Solution 4
(By user0003)
We plot the figure on a coordinate plane with $D=(0,0)$ and $A$ in the positive y-direction from the origin. If $Q_i=(k, 0)$ for some $k \neq 0$ , then the line $AQ_i$ can be represented as $y=-\frac{x}{k}+1$ . The intersection of this and $BD$ , which is the line $y=x$ , is
\[P_i = \left(\frac{k}{k+1}, \frac{k}{k+1}\right)\] .
As $Q_{i+1}$ is the projection of $P_i$ onto the x-axis, it lies at $\left(\frac{k}{k+1}, 0\right)$ . We have thus established that moving from $Q_i$ to $Q_{i+1}$ is equivalent to the transformation $x \rightarrow \frac{x}{x+1}$ on the x-coordinate. The closed form of of the x-coordinate of $Q_i$ can be deduced to be $\frac{1}{1+i}$ , which can be determined empirically and proven via induction on the initial case $Q_1 = \left(\frac{1}{2}, 0\right)$ . Now
\[[\Delta DQ_iP_i] = \frac{1}{2}(DQ_i)(Q_{i+1}P_i) = \frac{1}{2}(DQ_i)(DQ_{i+1}),\]
suggesting that $[\Delta DQ_iP_i]$ is equivalent to $\frac{1}{2(i+1)(i+2)}$ . The sum of this from $i=1$ to $\infty$ is a classic telescoping sequence as in Solution 1 and is equal to $\boxed{\textbf{(B) }\frac{1}{4}}$ .

## Solution 5 Diagram and Detailed Steps
Midpoint $Q_1$ of $\overline{CD}$ : $Q_1 = \left(\frac{1}{2}, 0\right)$
Equation of $\overline{AQ_1}$ : Slope $m = \frac{0 - 1}{\frac{1}{2} - 0} = -2$ Equation: $y = -2x + 1$
Line $\overline{BD}$ : - Equation: $y = x$
Intersection $P_1$ of $\overline{AQ_1}$ and $\overline{BD}$ :
Now, using the pattern for subsequent points $P_k$ and $Q_k$ :
General $Q_k$ - For $k \geq 1$ , $Q_k = \left(\frac{1}{k+1}, 0\right)$
Equation of $\overline{AQ_k}$ Slope $m = -(k+1)$ Equation: $y = -(k+1)x + 1$
Intersection $P_k$ of $\overline{AQ_k}$ and $\overline{BD}$ :
$Q_{k+1}$ is the foot of the perpendicular from $P_k$ to $\overline{CD}$ , so $Q_{k+1} = \left(\frac{1}{k+2}, 0\right)$
Area of $\triangle DQ_kP_k$ = $\frac{1}{2} \times DQ_k \times \text{Height}\ (y\ of\ P_{k+2})= \frac{1}{2} \times \frac{1}{k+1} \times \frac{1}{k+2} = \frac{1}{2} ( \frac{1}{k+1} - \frac{1}{k+2} )$
This recursive process confirms the telescoping series:
\[\sum_{k=1}^{\infty} \frac{1}{2(k+1)(k+2)} = \frac{1}{2} \left( \left( \frac{1}{2} - \frac{1}{3} \right) + \left( \frac{1}{3} - \frac{1}{4} \right) + \left( \frac{1}{4} - \frac{1}{5} \right) + \cdots \right)\]
Most terms cancel, and we are left with: $\frac{1}{2} \cdot \frac{1}{2} = \boxed{\textbf{(B) }\frac{1}{4}}$ .
~ luckuso

## Video Solution by CanadaMath (Problem 21-25)
https://www.youtube.com/watch?v=P3jJDLGyF2w&t=1546s
~THEMATHCANADIAN
### See Also
These problems are copyrighted © by the Mathematical Association of America.
These problems are copyrighted © by the Mathematical Association of America.
These problems are copyrighted © by the Mathematical Association of America.
These problems are copyrighted © by the Mathematical Association of America .