# 2001 AMC 8 Problem 12

## Problem

If $a\otimes b = \dfrac{a + b}{a - b}$ , then $(6\otimes 4)\otimes 3 =$

$\text{(A)}\ 4 \qquad \text{(B)}\ 13 \qquad \text{(C)}\ 15 \qquad \text{(D)}\ 30 \qquad \text{(E)}\ 72$

## Solution 1
$6\otimes4=\frac{6+4}{6-4}=\frac{10}{2}=5$ . $5\otimes3=\frac{5+3}{5-3}=\frac{8}{2}=\boxed{\textbf{(A)}\ 4}$

## Solution 2 (Overkill)
When you expand the general form of $(a\otimes b)\otimes c$ , you get \[(a\otimes b)\otimes c = \dfrac{a\otimes b + c}{a\otimes b - c}\] \[(a\otimes b)\otimes c = \dfrac{\dfrac{a + b}{a - b} + c}{\dfrac{a + b}{a - b} - c}\] \[(a\otimes b)\otimes c = \dfrac{\dfrac{a + b + ac - bc}{a - b}}{\dfrac{a + b - ac + bc}{a - b}}\] \[(a\otimes b)\otimes c = \dfrac{a + b + ac -bc}{a + b - ac + bc}\]
Now, substituting $a=6$ , $b=4$ , and $c=3$ :
\[(6\otimes 4)\otimes 3 = \dfrac{6 + 4 + 18 - 12}{6 + 4 - 18 + 12}\] \[(6\otimes 4)\otimes 3 = \dfrac{16}{4}\] \[(6\otimes 4)\otimes 3 = 4\] $\boxed{\text {(A)}}$
~megaboy6679

## Video Solution-Cooler Method
https://www.youtube.com/watch?v=ZfwtAiH_6PI&t=36s
### See Also