# 2023 AMC 12A Problem 19

## Problem

What is the product of all solutions to the equation \[\log_{7x}2023\cdot \log_{289x}2023=\log_{2023x}2023\]

$\textbf{(A) } (\log_{2023}7\cdot \log_{2023}289)^2\qquad\textbf{(B) } \log_{2023}7\cdot \log_{2023}289\qquad\textbf{(C) } 1 \\ \qquad \textbf{(D) } \log_{7}2023\cdot \log_{289}2023\qquad \textbf{(E) } (\log_7 2023\cdot\log_{289} 2023)^2$

## Solution 1
For $\log_{7x}2023\cdot \log_{289x}2023=\log_{2023x}2023$ , transform it into $\dfrac{\ln 289+\ln 7}{\ln 7 + \ln x}\cdot \dfrac{\ln 289+\ln 7}{\ln 289 + \ln x}=\dfrac{\ln 289+\ln 7}{\ln 289+\ln 7+\ln x}$ . Replace $\ln x$ with $y$ . Because we want to find the product of all solutions of $x$ , it is equivalent to finding the exponential of the sum of all solutions of $y$ . Change the equation to standard quadratic equation form, the term with 1 power of $y$ is canceled. By using Vieta, we see that since there does not exist a $by$ term, $\sum y=0$ and $\prod x=e^0=\boxed{\textbf{(C)} 1}$ .
~plasta

## Solution 2 (Same idea as Solution 1 with easily understood steps)
\[\log_{7x}2023\cdot \log_{289x}2023=\log_{2023x}2023\]
Rearranging it give us:
\[\log_{2023}7x\cdot \log_{2023}289x=\log_{2023}2023x\]
\[(\log_{2023}7+\log_{2023}x)(\log_{2023}289+\log_{2023}x)=(\log_{2023}2023+\log_{2023}x)\]
let $\log_{2023}x$ be $a$ , we get
\[(\log_{2023}7+a)(\log_{2023}289+a)=1+a\]
\[a^2+(\log_{2023}7+\log_{2023}289)a+\log_{2023}7 \cdot \log_{2023}289=1+a\]
\[a^2+\log_{2023}7 \cdot \log_{2023}289-1=0\]
by Vieta's Formulas,
\[a_1+a_2=0\]
\[\log_{2023}{x_1}+\log_{2023}{x_2}=0\]
\[\log_{2023}{x_1x_2}=0\]
\[x_1x_2=\boxed{\textbf{(C)} 1}\]
~lptoggled ～edited by DRA777

## Solution 3
Similar to solution 1, change the bases first \[\frac{\ln 289+\ln 7}{\ln7 + \ln{x}} \cdot \frac{\ln 289+\ln 7}{2\ln17 + \ln{x}} = \frac{\ln 289+\ln 7}{\ln7 + 2\ln17 + \ln{x}}\] Cancel and cross multiply to get \[(\ln7 + 2\ln17)(\ln7 + 2\ln17 + \ln{x}) = (\ln7 + \ln{x})(2\ln17 + \ln{x})\] Simplify to get \[(\ln{x})^2 = 4(\ln17)^2 + 2\ln17\ln7 + (\ln7)^2\] \[\ln{x} = \pm \sqrt{4(\ln17)^2 + 2\ln17\ln7 + (\ln7)^2}\] The sum of all possible $\ln{x}$ is 0, thus the product of all solutions of $x$ is $\boxed{\textbf{(C)} 1}$
~dwarf_marshmallow

## Solution 4(Fakesolve)
We take the reciprocal of both sides: \[\frac{1}{\log_{7x}2023}\cdot \frac{1}{\log_{289x}2023}=\frac{1}{\log_{2023x}2023}.\] Using logarithm properties, we have \[\log_{2023}7x\cdot \log_{2023}289x=\log_{2023}2023x.\] Simplify to obtain \[2023x^2=2023x,\] from which we have $x=\boxed{\textbf{(C)} 1}$
~MLiang2018
This solution works for this problem by chance but do note that the simplification step to get \[2023x^2=2023x\] is not how log properties work and that the actual solutions for x are \[x = e^{ \pm \sqrt{ln^2(7)+ln(17)ln(2092529)}}\] (as shown in solution 3) which multiply to 1
~silk-hyacinth

## Solution 5(Similar to solution 4, Fakesolve)
First, we take the reciprocal of both sides. We get \[\frac{1}{\log_{7x}2023}\cdot \frac{1}{\log_{289x}2023}=\frac{1}{\log_{2023x}2023}.\] Flip the logarithms to get \[\log_{2023}7x\cdot \log_{2023}289x=\log_{2023}2023x.\]
Now we can use $\log_{a}bc=\log_{a}b+\log_{a}c$ . We get \[\log_{2023}7+\log_{2023}x+\log_{2023}289+\log_{2023}x=\log_{2023}2023+\log_{2023}x.\] The $\log_{2023}7+\log_{2023}289$ and $\log_{2023}2023$ terms cancel, giving \[2\cdot\log_{2023}x=\log_{2023}x\] so now we are sure that $\log_{2023}x=0$ , so the only solution is $x=\boxed{\textbf{(C)} 1}$ .
~Yrock

## Solution 6 (Bogus Solution)
We can begin by changing the logarithms' base to $x$ and simplifying: $\newline$ $\frac{(\log_{x} 2023)^2}{\log_{x} 7 +1} \cdot \frac{1}{\log_{x} 289 + 1} = 1$ $\newline$ After that, we can multiply the denominator on the $\text{LHS}$ on both sides, resulting in: $\newline$ $(\log_{x} 2023)^2 = (\log_{x} 7 +1)(\log_{x} 289 +1)$ $\newline$ $(\log_{x} 2023)^2 = \log_{x} 2023 + \log_{x} 7 + \log_{x} 289 + 1$ $\newline$ $(\log_{x} 2023)^2 = 2\log_{x} 2023 + 1$ $\newline$ Now, we can substitute some variable $a$ as $\log_{x} 2023$ , giving the quadratic $a^2-2a-1=0$ . By Vieta's, the product of the roots is $1$ , thus the solution is $\boxed{\textbf{(C)} 1}$ .
~cyberhacker

## Video Solution 1 by OmegaLearn
https://youtu.be/OcNU62SMh4o

## Video Solution
https://youtu.be/-CZkFE-wriQ
~Steven Chen (Professor Chen Education Palace, www.professorchenedu.com)
These problems are copyrighted © by the Mathematical Association of America.
These problems are copyrighted © by the Mathematical Association of America.
These problems are copyrighted © by the Mathematical Association of America.
These problems are copyrighted © by the Mathematical Association of America .