# 2023 AMC 12A Problem 9

## Problem

A square of area $2$ is inscribed in a square of area $3$ , creating four congruent triangles, as shown below. What is the ratio of the shorter leg to the longer leg in the shaded right triangle? [asy] size(200); defaultpen(linewidth(0.6pt)+fontsize(10pt)); real y = sqrt(3); pair A,B,C,D,E,F,G,H; A = (0,0); B = (0,y); C = (y,y); D = (y,0); E = ((y + 1)/2,y); F = (y, (y - 1)/2); G = ((y - 1)/2, 0); H = (0,(y + 1)/2); fill(H--B--E--cycle, gray); draw(A--B--C--D--cycle); draw(E--F--G--H--cycle); [/asy]

$\textbf{(A) }\frac15\qquad\textbf{(B) }\frac14\qquad\textbf{(C) }2-\sqrt3\qquad\textbf{(D) }\sqrt3-\sqrt2\qquad\textbf{(E) }\sqrt2-1$

## Solution 1
The side lengths of the inner square and outer square are $\sqrt{2}$ and $\sqrt{3}$ respectively. Let the shorter side of our triangle be $x$ , thus the longer leg is $\sqrt{3}-x$ . Hence, by the Pythagorean Theorem, we have \begin{align*} (\sqrt{3}-x)^2+x^2&=(\sqrt{2})^2 \\ 3-2\sqrt{3}x+x^2+x^2&=2 \\ 2x^2-2\sqrt{3}x+1&=0. \end{align*} By the quadratic formula, we find that $x=\frac{\sqrt{3}\pm1}{2}$ , so the answer is $\frac{\sqrt{3}-1}{\sqrt{3}+1}=\boxed{\textbf{(C) }2-\sqrt3}.$
~semisteve ~SirAppel ~ItsMeNoobieboy

## Solution 2 (Area)
Looking at the diagram, we know that the square inscribed in the square with area $3$ has area $2$ . Thus, the area outside of the small square is $3-2=1.$ This area is composed of $4$ congruent triangles, so we know that each triangle has an area of $\dfrac14$ .
From solution $1$ , the base (short side of the triangle) has a length $x$ and the height $\sqrt{3} - x$ , which means that $\frac{x\left(\sqrt{3} - x\right)}{2} = \frac{1}{4}$ .
We can turn this into a quadratic equation: $x^2-x\sqrt{3}+\frac{1}{2} = 0$ .
By using the quadratic formula, we get $x=\frac{\sqrt{3}\pm1}{2}$ .Therefore, the answer is $\frac{\sqrt{3}-1}{\sqrt{3}+1}=\boxed{\textbf{(C) }2-\sqrt3}.$
~ghfhgvghj10 (If I made any mistakes, feel free to make minor edits)
(Clarity & formatting edits by Technodoggo)

## Solution 3
Let $x$ be the ratio of the shorter leg to the longer leg, and $y$ be the length of longer leg. The length of the shorter leg will be $xy$ .
Because the sum of two legs is the side length of the outside square, we have $xy + y = \sqrt{3}$ , which means $(xy)^2 + y^2 + 2xy^2 = 3$ . Using the Pythagorean Theorem for the shaded right triangle, we also have $(xy)^2 + y^2 = 2$ . Solving both equations, we get $2xy^2 = 1$ . Using $y^2=\frac{1}{2x}$ to substitute $y$ in the second equation, we get $x^2\cdot \frac{1}{2x} + \frac{1}{2x} = 2$ . Hence, $x^2 - 4x + 1 = 0$ . By using the quadratic formula, we get $x=2\pm \sqrt3$ . Because $x$ be the ratio of the shorter leg to the longer leg, it is always less than $1$ . Therefore, the answer is $\boxed{\textbf{(C) }2-\sqrt3}$ .
~sqroot

## Solution 4
The side length of the bigger square is equal to $\sqrt{3}$ , while the side length of the smaller square is $\sqrt{2}$ . Let $x$ be the shorter leg and $y$ be the longer one. Clearly, $x+y=\sqrt{3}$ , and $xy=\frac{1}{2}$ . Using Vieta's to build a quadratic, we get \[x^2-\sqrt{3}x+\frac{1}{2}=0.\] Solving, we get $x=\frac{\sqrt{3}-1}{2}$ and $y=\frac{\sqrt{3}+1}{2}$ . Thus, we find $\frac{x}{y}=\frac{\sqrt{3}-1}{\sqrt{3}+1}=\frac{(\sqrt{3}-1)^2}{(\sqrt{3}+1)\cdot(\sqrt{3}-1)}=\frac{4-2\sqrt{3}}{2}=\boxed{\textbf{(C) }2-\sqrt3}$ .
~vadava_lx

## Solution 5
Let $\theta$ be the angle opposite the smaller leg. We want to find $\tan\theta$ .
The area of the triangle is $\frac{1}{2}\left(\sqrt{2}\sin\theta\right)\left(\sqrt{2}\cos\theta\right)=\frac{1}{2}\sin 2\theta=\frac{1}{4},$ which implies $\sin 2\theta = \frac{1}{2},$ or $\theta=15^\circ$ . Therefore $\tan \theta = \boxed{\textbf{(C) }2-\sqrt3}$

## Solution 6
Allow a and b to be the sides of a triangle. WLOG, suppose $a > b.$ We want to find $\frac{b}{a}$ . Notice that the area of a triangle is $\frac{3-2}{4}$ , which results in $\frac{1}{4}$ . Thus, $ab = \frac{1}{2}$ . However, the square of the hypotenuse of this triangle is $a^2+b^2$ , but also $2$ . We can write $b$ as $\frac{1}{2a}$ , and then plug it in. We get $a^2+\frac{1}{4a^2} = 2$ , so $4a^4-8a^2+1 = 0$ . Applying the quadratic formula, $a^2 = \frac{8 \pm 4\sqrt{3}}{2}$ , or $4 \pm 2\sqrt3$ . However, since $a$ and $b$ must both be solutions of the quadratic, since both equations were cyclic. Since $a>b$ , then $a^2 = 4+2\sqrt3$ , and $b^2 = 4-2\sqrt3$ . To find $\frac{b}{a}$ , we can simply find the square root of $\frac{b^2}{a^2}$ . This is $\sqrt{\frac{4-2\sqrt3}{4+2\sqrt3}} = \sqrt{\frac{2-\sqrt3}{2+\sqrt3}} = \sqrt{(2-\sqrt3)(2-\sqrt3)} = \boxed {2-\sqrt3}$ , so the answer is $\boxed {C}$ . - Sepehr2010

## Solution 7 (Manipulation)
Let $a$ be the length of the shorter leg and $b$ be the longer leg. By the Pythagorean theorem, we can derive that $a^2+b^2=2$ . Using area we can also derive that $2ab=1$ . $(a+b)^2=3$ as given in the diagram, we can find that $(a-b)^2=1$ because $4ab=2$ . This means that $b+a=\sqrt{3}$ and $b-a=1$ . Adding the equations gives $b=\frac{\sqrt{3}+1}{2}$ and when $b$ is plugged in $a = \frac{\sqrt{3}-1}{2}$ . Rationalizing the denominators gives us $\boxed{\textbf{(C) } 2-\sqrt{3}}$ .

## Solution 8
Let $s$ be the length of the shorter leg, $l$ the longer leg, and $t$ the desired ratio. We have: \[s^2+l^2=2 \text{ and } \frac{1}{2}sl=\frac{1}{4}\] The former dividing the latter gives: \[t+\frac{1}{t}=4\] Solve this for $t$ .
~ yinglinwu

## Video Solution by Little Fermat
https://youtu.be/h2Pf2hvF1wE?si=jPmOlhD8haZA8-hK&t=2309 ~little-fermat

## Video Solution by Math-X (First understand the problem!!!)
https://youtu.be/GP-DYudh5qU?si=H7rtzYDnG-hbDpIQ&t=2706
~Math-X

## Video Solution by Power Solve (easy to digest!)
https://www.youtube.com/watch?v=7KXT1pI-i64

## Video Solution (üêâ‚ö°Under 5 min‚ö°üêâ)
https://youtu.be/OiBUPU1bULc
~Education, the Study of Everything

## Video Solution by CosineMethod [üî•Fast and Easyüî•]
https://www.youtube.com/watch?v=IVgzVS86Ogo

## Video Solution
https://youtu.be/jL2k7MFgfzQ
~Steven Chen (Professor Chen Education Palace, www.professorchenedu.com)
### See Also
These problems are copyrighted ¬© by the Mathematical Association of America.
These problems are copyrighted ¬© by the Mathematical Association of America.
These problems are copyrighted ¬© by the Mathematical Association of America.
These problems are copyrighted ¬© by the Mathematical Association of America .