# 2023 AMC 12A Problem 10

## Problem

Positive real numbers $x$ and $y$ satisfy $y^3=x^2$ and $(y-x)^2=4y^2$ . What is $x+y$ ? $\textbf{(A) }12\qquad\textbf{(B) }18\qquad\textbf{(C) }24\qquad\textbf{(D) }36\qquad\textbf{(E) }42$

## Solution 1
Because $y^3=x^2$ , set $x=a^3$ , $y=a^2$ ( $a\neq 0$ ). Put them in $(y-x)^2=4y^2$ we get $(a^2(a-1))^2=4a^4$ which implies $a^2-2a+1=4$ . Solve the equation to get $a=3$ or $-1$ . Since $x$ and $y$ are positive, $a=3$ and $x+y=3^3+3^2=\boxed{\textbf{(D)} 36}$ .
~plasta

## Solution 2
Let's take the second equation and square root both sides. This will obtain $y-x = \pm2y$ . Solving the case where $y-x=+2y$ , we'd find that $x=-y$ . This is known to be false because both $x$ and $y$ have to be positive, and $x=-y$ implies that at least one of the variables is not positive. So we instead solve the case where $y-x=-2y$ . This means that $x=3y$ . Inputting this value into the first equation, we find $y^3 = (3y)^2$ , from which $y=9$ .
This means that $x=3y=3(9)=27$ . Therefore, $x+y=9+27=\boxed{36}$
~lprado

## Solution 3: Quadratic formula
first expand
$(y-x)^2 = 4y^2$
$y^2-2xy+x^2 = 4y^2$
$y^2-2yx+x^2 = 4y^2$
$x^2-2xy-3y^2 = 0$
$x=\frac{-b\pm\sqrt{b^2-4ac}}{2a}$
consider a=1 b=-2y c=-3y^2
$x=\frac{2y\pm\sqrt{(-2y)^2-4(1)(-3y^2)}}{2a}$
$x=\frac{2y\pm\sqrt{16y^2}}{2a}$
$\frac{2y+4y}{2}$ or $\frac{2y-4y}{2}$
$x=y+2y$ and $x=y-2y$
$x=3y$ and $x=-y$
we can see both x and y will be postive in $x=3y$
now do same as solution 2 \[y^3 = (3y)^2\] \[y^3 = 9y^2\] \[y=9\] This means that $x=3y=3(9)=27$ . Therefore, $x+y=9+27=\boxed{36}$
alternate solving similar to solution 5(~soapedya): you can also factor at $x^2-2xy-3y^2 = 0$ into $(x-3y)(x+y) = 0$
Since $x+y = 0$ would result in one of them being negative (or just look at the answer choices; it is not 0), $x-3y = 0$ so $x = 3y$ . plugging back into $y^3 = x^2$ gives $y = 9$ and then $x=27$ , so $x+y$ is $\boxed{36}$ .

## Solution 4: Substitution
Since $a^2 = |a|^2$ , we can rewrite the second equation as $(x-y)^2=4y^2$
Let $u=x+y$ . The second equation becomes
\[(u-2y)^2 = 4y^2\] \[u^2 - 4uy = 0\] \[u = 4y\] \[x+y = 4y\] \[x = 3y.\]
Substituting this into the first equation, we have
\[y^3 = (3y)^2,\] so $x = 9$ .
Hence $x = 27$ and $x + y = \boxed{\textbf{(D)} 36}.$
-Benedict T (countmath1)

## Solution 5: Difference of Squares
We will use the difference of squares in the second equation.
\[(y-x)^2=4y^2\] \[(y-x)^2-(2y)^2=0\] \[(y-x-2y)(y-x+2y)=0\] \[-(x+y)(3y-x)=0\]
Since x and y are positive, x+y is non-zero. Thus, \[3y=x\] .
Substituting into the first equation:
\[y^3=x^2\] \[y^3=9y^2\] \[y=9, x=27 \rightarrow x+y=\boxed{\textbf{(D)} 36}\]

## Video Solution (easy to digest) by Power Solve
https://youtu.be/YXIH3UbLqK8?si=ia236Rh1UU681RNT&t=1279

## Video Solution (⚡ Under 3 minutes ⚡)
https://youtu.be/G63hRr9bkzI
~Education, the Study of Everything

## Video Solution
https://youtu.be/OqlerYo-uPU
~Steven Chen (Professor Chen Education Palace, www.professorchenedu.com)
These problems are copyrighted © by the Mathematical Association of America.
These problems are copyrighted © by the Mathematical Association of America.
These problems are copyrighted © by the Mathematical Association of America.
These problems are copyrighted © by the Mathematical Association of America .