# 2024 AMC 12A Problem 13

## Problem

The graph of $y=e^{x+1}+e^{-x}-2$ has an axis of symmetry. What is the reflection of the point $(-1,\tfrac{1}{2})$ over this axis?

$\textbf{(A) }\left(-1,-\frac{3}{2}\right)\qquad\textbf{(B) }(-1,0)\qquad\textbf{(C) }\left(-1,\frac{1}{2}\right)\qquad\textbf{(D) }\left(0,\frac{1}{2}\right)\qquad\textbf{(E) }\left(3,\frac{1}{2}\right)$

## Solution 1
The line of symmetry is probably of the form $x=a$ for some constant $a$ . A vertical line of symmetry at $x=a$ for a function $f$ exists if and only if $f(a-b)=f(a+b)$ ; we substitute $a-b$ and $a+b$ into our given function and see that we must have
\[e^{a-b+1}+e^{-(a-b)}-2=e^{a+b+1}+e^{-(a+b)}-2\]
for all real $b$ . Simplifying:
\begin{align*} e^{a-b+1}+e^{-(a-b)}-2&=e^{a+b+1}+e^{-(a+b)}-2 \\ e^{a-b+1}+e^{b-a}&=e^{a+b+1}+e^{-a-b} \\ e^{a-b+1}-e^{-a-b}&=e^{a+b+1}-e^{b-a} \\ e^{-b}\left(e^{a+1}-e^{-a}\right)&=e^b\left(e^{a+1}-e^{-a}\right). \\ \end{align*}
If $e^{a+1}-e^{-a}\neq0$ , then $e^{-b}=e^b$ for all real $b$ ; this is clearly impossible, so let $e^{a+1}-e^{-a}=0\implies a+1=-a\implies a=-\dfrac12$ . Thus, our line of symmetry is $x=-\dfrac12$ , and reflecting $\left(-1,\dfrac12\right)$ over this line gives $\boxed{\textbf{(D) }\left(0,\dfrac12\right)}.$
~Technodoggo

## Solution 2 (Graphing)
Consider the graphs of $y=e^{x+1}-1$ and $y=e^{-x}-1$ . A rough sketch will show that they intercept somewhere between -1 and 0 and the axis of symmetry is vertical. Thus, $\boxed{\textbf{(D) }\left(0,\dfrac12\right)}$ is the only possible answer.
Note: You can more rigorously think about the solution by noting that since the derivative of the power that e is raised to in one equation is equal to the derivative of the power that e is raised to multiplied by $-1$ and both equations are subtracted by 1, then the sum of both equations will be the same from one side of the interception to the other. Setting both equations equal to each other, it is trivial to see $x=-1/2$ , giving us the axis of symmetry.
~woeIsMe
[asy] unitsize(2cm); real e = 2.71828; real f1(real x) {return e^(x+1)-1;} real f2(real x) {return e^(0-x)-1;} draw(graph(f1,-1.5,0.5)); draw(graph(f2,-1.5,0.5)); xaxis(-2,1,Ticks()); yaxis(f2(0.5),f1(0.5),Ticks()); draw((-0.5,f2(0.5))--(-0.5,f1(0.5)),red+dashed); /*graph by Technodoggo, 9 November 2024*/ [/asy] (graph by Technodoggo)

## Solution 3 (Derivatives)
Since y is a proper function of x, the axis of symmetry is vertical (and so answer choices A and B are impossible). Where a function crosses a vertical axis of symmetry, it must have either a vertical asymptote (clearly impossible for this given function, since linear functions and exponential function are total functions) or a local maximum or minimum (derivative 0).
So the derivative is equal to 0: $\frac{d[e^{x+1}+e^{-x}-2]}{dx} = 0 = e^{x+1}-e^{-x}$
To solve for $x$ , make a substitution: $u = e^x$ $0 = e*u - \frac{1}{u}$ -> $0 = \frac{e*u^2 - 1}{u}$ -> $0 = e*u^2 - 1$ -> $e*u^2 = 1$ -> $(e^x)^2 = \frac{1}{e}$ -> $e^{2x} = e^{-1}$ -> $2x = -1$ -> $x = -\frac{1}{2}$
Reflect $\left(-1, \frac{1}{2}\right)$ over $x = -\frac{1}{2}$ , giving answer choice $\boxed{\textbf{(D) }\left(0,\dfrac12\right)}.$

## Solution 4
\[f(0) = e-1\] \[f(1) = e^2 + e^{-1} - 2\] \[f(-1) = 1+ e -2 = e-1\] \[f(-2) = e^{-1} + e^2 -2\]
so f(0) = f(-1) , f(1) =f(-2) then f(x) is symmetric about x=-1/2 point (-1, 1/2) reflects over axis x=-1/2 is point ( 0, 1/2) answer choice D ~ luckuso

## Solution 5
Notice that this is simply a transformation of $\cosh(x)$ , specifically $2e^\frac{1}{2}\cosh(x + \frac{1}{2}) + 2$ . We know that $\cosh(x)$ has a parabolic shape with an axis of symmetry $x=0$ . Since this is simple a transformation of $\frac{1}{2}$ to the left of the origin, we have the axis of symmetry is $x = -\frac{1}{2}$ giving us $\boxed{\textbf{(D) }\left(0,\dfrac12\right)}$
~KEVIN_LIU

## Solution 5 (Graph)
~ luckuso

## Solution 6
\[f(-x-1) = e^{-x-1+1} + e^{-(-x-1)} - 2 = e^{-x} + e^{x+1} - 2 = f(x)\]
So the axis is $\frac{x + (-x - 1)}{2} = -1/2$
Point $(-1, 1/2)$ reflects over the axis $x=-1/2$ to the point $\boxed{\textbf{(D) }\left(0,\dfrac12\right)}$
~ luckuso

## Solution 7
Setting the axis of symmetry as $x=a$ implies $f(2a-x) = f(x)$
\begin{align*} f(2a-x) &= f(x) \\ e^{2a-x+1} + e^{-(2a-x)} - 2 &= e^{x+1} + e^{-x} - 2 \end{align*}
Analyzing the terms $e^{2a-x+1}$ and $e^{-x}$ tells us that $2a+1 = 0$
This reveals that $a = -1/2$
Finally, point $(-1, 1/2)$ reflected over the axis $x=-1/2$ is the point $\boxed{\textbf{(D) }\left(0,\dfrac12\right)}$
~ luckuso

## Solution 8
First identify that the graphs are both forms of the parent function $e^x$ and will not have a slant asymptote, so we can eliminate answer choices with a different y-value and the same x-value as this function can not have different y value for a same x value.
The answer choices that we can still consider are: $\qquad\textbf{(D) }\left(0,\frac{1}{2}\right)\qquad\textbf{(E) }\left(3,\frac{1}{2}\right)$
Remember that the constant term does not matter for an axis of symmetry, as it simply shifts the function(s) up or down.
Hence, we can use the answer choices and plug in valid values of $x$ for $e^{x+1}=e^{-x}$ .
The answer for $x$ is then ${-1/2}$ , and the answer is $\boxed{\textbf{(D) }\left(0,\dfrac12\right)}$
~ Aaron_Q
These problems are copyrighted © by the Mathematical Association of America.
These problems are copyrighted © by the Mathematical Association of America.
These problems are copyrighted © by the Mathematical Association of America.
These problems are copyrighted © by the Mathematical Association of America .