# 2018 AMC 10A Problem 10

## Problem

Suppose that real number $x$ satisfies \[\sqrt{49-x^2}-\sqrt{25-x^2}=3\] What is the value of $\sqrt{49-x^2}+\sqrt{25-x^2}$ ?

$\textbf{(A) }8\qquad \textbf{(B) }\sqrt{33}+8\qquad \textbf{(C) }9\qquad \textbf{(D) }2\sqrt{10}+4\qquad \textbf{(E) }12\qquad$

## Solution 1
We let $a=\sqrt{49-x^2}+\sqrt{25-x^2}$ ; in other words, we want to find $a$ . We know that $a\cdot3=\left(\sqrt{49-x^2}+\sqrt{25-x^2}\right)\cdot\left(\sqrt{49-x^2}-\sqrt{25-x^2}\right)=\left(\sqrt{49-x^2}\right)^2-\left(\sqrt{25-x^2}\right)^2=\left(49-x^2\right)-\left(25-x^2\right)=24.$ Thus, $a=\boxed{8}$ .
~Technodoggo
Alternative method: Let $a=\sqrt{49-x^2}+\sqrt{25-x^2}$ , $b=\sqrt{49-x^2}-\sqrt{25-x^2}$ . $a*b=49-x^2 - 25 + x^2 = 24$ . The problem states that $b=3$ , so we get $a = 24 / 3 = 8$ . The answer is $\boxed{\textbf{(A) }8}$ .
~SwordAxe

## Solution 2
Let $a = \sqrt{49-x^2}$ , and $b = \sqrt{25-x^2}$ . Solving for the constants in terms of $x$ , $a$ , and $b$ , we get $a^2 + x^2 = 49$ , and $b^2 + x^2 = 25$ . Subtracting the second equation from the first gives us $a^2 - b^2 = 24$ . Difference of squares gives us $(a+b)(a-b) = 24$ . Since we want to find $a+b = \sqrt{49-x^2}+\sqrt{25-x^2}$ , and we know $a-b = 3$ , we get $3(a+b) = 24$ , so $a+b = \boxed{\textbf{(A) }8}$
~idk12345678

## Solution 3
We can substitute $25 - x^2$ for $a$ , thus turning the equation into $\sqrt{a+24} - \sqrt{a} = 3$ . Moving the $\sqrt{a}$ to the other side and squaring gives us $a + 24 = 9 + 6\sqrt{a} + a$ , solving for $a$ gives us 25/4. We substitute this value into the expression they asked us to evaluate giving 8.
~ SAMANTAP

## Solution 4
Move $-\sqrt{25-x^2}$ to the right to get $\sqrt{49-x^2} = 3 + \sqrt{25-x^2}$ . Square both sides to get $49-x^2 = 9 + 6\sqrt{25-x^2} + (25-x^2)$ . Simplify to get $15 = 6\sqrt{25-x^2}$ , or $\frac{5}{2} = \sqrt{25-x^2}$ Substitute this back into the original equation tog et that $\sqrt{49-x^2} = \frac{11}{2}$ . The answer is $\boxed{\textbf{(A) }8}$

## Solution 5(Jaideep's Difference of Roots Equals Integer Method)[JDRIM]
We are given that, $\sqrt(49-x^2) - \sqrt(25-x^2) = 3$ We are asked to find, $\sqrt(49-x^2) + \sqrt(25-x^2)$ Notice that these two expressions are conjugates of one another. Therefore, we can find that by multiply these two conjugates by one another we should be able to find that: $(\sqrt(49-x^2) - \sqrt(25-x^2))(\sqrt(49-x^2) + \sqrt(25-x^2)) = (49-x^2) - (25-x^2)$ $\Rightarrow 49-x^2-25+x^2 = 24$ We are already given that the first expression equals 3, thus, our expression now becomes: $3(\sqrt(49-x^2)+\sqrt(25-x^2)) = 24$ $\Rightarrow \sqrt(49-x^2)+\sqrt(25-x^2) = 8$ Thus, the answer is $\boxed{\textbf{(A) }8}$
~im_space_cadet

## Solution 6 (Fast version of solution 1)
Let \( x = \sqrt{49-x^2} \) and \( y = \sqrt{25-x^2} \). Then, we have (1) \( x - y = 3 \) and \( x^2 = y^2 + 24 \) or (2) \( x^2 - y^2 = 24 \). Notice that \( x^2 - y^2 = (x + y)(x - y) \). So, dividing (1) by (2), we get that \( x + y = \sqrt{49 - x^2} + \sqrt{25 - x^2} = \frac{24}{3} = 8 \).
~maxd3

## Video Solution (HOW TO THINK CREATIVELY!)
https://youtu.be/P-atxiiTw2I
~Education, the Study of Everything

## Video Solutions

## Video Solution 1
https://youtu.be/ba6w1OhXqOQ?t=1403
~ pi_is_3.14

## Video Solution 2
https://youtu.be/zQG70XKAdeA ~ North America Math Contest Go Go Go

## Video Solution 3
https://youtu.be/ZiZVIMmo260

## Video Solution 4
https://youtu.be/5cA87rbzFdw
~savannahsolver
### See Also