# 2022 AMC 10A Problem 6

## Problem

Which expression is equal to \[\left|a-2-\sqrt{(a-1)^2}\right|\] for $a<0?$

$\textbf{(A) } 3-2a \qquad \textbf{(B) } 1-a \qquad \textbf{(C) } 1 \qquad \textbf{(D) } a+1 \qquad \textbf{(E) } 3$

## Solution 1
We have \begin{align*} \left|a-2-\sqrt{(a-1)^2}\right| &= \left|a-2-|a-1|\right| \\ &=\left|a-2-(1-a)\right| \\ &=\left|2a-3\right| \\ &=\boxed{\textbf{(A) } 3-2a}. \end{align*} ~MRENTHUSIASM

## Solution 2
Assume that $a=-1.$ Then, the given expression simplifies to $5$ : \begin{align*} \left|a-2-\sqrt{(a-1)^2}\right| &= \left|-1-2-\sqrt{(-1-1)^2}\right| \\ &= \left|-1-2-\sqrt{4}\right| \\ &= \left|-1-2-2\right| \\ &= 5. \end{align*} Then, we test each of the answer choices to see which one is equal to $5$ :
$\textbf{(A) } 3-2a = 3-2\cdot(-1) = 3+2 = 5.$
$\textbf{(B) } 1-a = 1-(-1) = 2 \neq 5.$
$\textbf{(C) } 1 \neq 5.$
$\textbf{(D) } a+1 = -1+1 = 0 \neq 5.$
$\textbf{(E) } 3 \neq 5.$
The only answer choice equal to $5$ for $a=-1$ is $\boxed{\textbf{(A) } 3-2a}.$
-MathWizard09

## Solution 3
The given function is continuous, so assume that $a=0.$ Then, the given expression simplifies to $3.$
We test each of the answer choices and get $\textbf{(A) } 3-2a$ or $\textbf{(E) } 3.$
We test $x = - 1000$ and get $\left|-1000-2- \text{positive} \right| \ne 3 \implies \boxed{\textbf{(A) } 3-2a}.$
vladimir.shelomovskii@gmail.com, vvsss

## Solution 4
We know that ,
\(\begin{aligned} & |x|=x, \text { if } x>0 \\ & =-x, \text { if } x<0 \\ & \text { Now, }\left|a-2-\sqrt{(a-1)^2}\right|=\left|a-2-\sqrt{(1-a)^2}\right|, \text { as } a<0 \\ & =|a-2-(1-a)| \\ & =|2 a-3| \\ & =-(2 a-3) \text { as } a<0 \\ & =3-2 a\end{aligned}\)
So, the correct choice is option $\boxed{\textbf{(A) } 3-2a}.$
~KENJAKURA

## Solution 5
Because the degree of the expression is $1$ , and all the solutions are of degree $1$ or $0$ , we can assume the function is linear for $a<0$ and try values to find what the function is.
We can first say from Solution 1 that: \[\left|a-2-\sqrt{(a-1)^2}\right| = \left|a-2-|a-1|\right|\] Then, we can try values: \begin{array}{cccc} a & \text{Plug in values} & = & \text{Result} \\ \hline -1 & \left|-1-2-\left|-1-1\right|\right| & = & \left|-3-2\right| = 5 \\ -2 & \left|-2-2-\left|-2-1\right|\right| & = & \left|-4-3\right| = 7 \\ -3 & \left|-3-2-\left|-3-1\right|\right| & = & \left|-5-4\right| = 9 \\ \end{array} We can see that this is a linear function. We can find that the slope is $m = \frac{7-5}{-2-(-1)} = \frac{2}{-1} = -2.$ Using the first pair: \begin{aligned} y & = mx+b \\ 5 & = -2(-1)+b \\ 5 & = 2+b \\ 3 & = b \\ y & = -2x+3 \\ \end{aligned}
We take that $y$ equals the expression, and $x$ is $a$ . This gives $-2a+3$ , or $3-2a$ . Testing to make sure the answer is correct (like that in Solution 2) is a good practice to have and shows that the correct choice must be $\boxed{\textbf{(A) } 3-2a}.$
~Eugenius

## Video Solution 1 (Quick and Easy)
https://youtu.be/ZWHzdrW4rvw
~Education, the Study of Everything

## Video Solution 2
https://youtu.be/XWTTtL9kW98
### See Also
These problems are copyrighted © by the Mathematical Association of America.
These problems are copyrighted © by the Mathematical Association of America.
These problems are copyrighted © by the Mathematical Association of America.
These problems are copyrighted © by the Mathematical Association of America .