# 2023 AMC 12B Problem 23

## Problem

When $n$ standard six-sided dice are rolled, the product of the numbers rolled can be any of $936$ possible values. What is $n$ ?

$\textbf{(A)}~11\qquad\textbf{(B)}~6\qquad\textbf{(C)}~8\qquad\textbf{(D)}~10\qquad\textbf{(E)}~9$

## Solution 1
We start by trying to prove a function of $n$ , and then we can apply the function and equate it to $936$ to find the value of $n$ .
It is helpful to think of this problem in the format $(1+2+3+4+5+6) \cdot (1+2+3+4+5+6) \dots$ . Note that if we represent the scenario in this manner, we can think of picking a $1$ for one factor and then a $5$ for another factor to form their product - this is similar thinking to when we have the factorized form of a polynomial. Unfortunately this is not quite accurate to the problem because we can reach the same product in many ways: for example for $n=2$ , $4$ can be reached by picking $1$ and $4$ or $2$ and $2$ . However, this form gives us insights that will be useful later in the problem.
Note that there are only $3$ primes in the set $\{1,2,3,4,5,6\}$ : $2,3,$ and $5$ . Thus if we're forming the product of possible values of a dice roll, the product has to be written in the form $2^h \cdot 3^i \cdot 5^j$ (the choice of variables will become clear later), for integer nonnegative values $h,i,j$ . So now the problem boils down to how many distinct triplets $(h,i,j)$ can be formed by taking the product of $n$ dice values.
We start our work on representing $j$ : the powers of $5$ , because it is the simplest in this scenario because there is only one factor of $5$ in the set. Because of this, having $j$ fives in our prime factorization of the product is equivalent to picking $j$ factors from the polynomial $(1+\dots + 6) \cdots$ and choosing each factor to be a $5$ . Now that we've selected $j$ factors, there are $n-j$ factors remaining to choose our powers of $3$ and $2$ .
Suppose our prime factorization of this product contains $i$ powers of $3$ . These powers of $3$ can either come from a $3$ factor or a $6$ factor, but since both $3$ and $6$ contain only one power of $3$ , this means that a product with $i$ powers of $3$ corresponds directly to picking $i$ factors from the polynomial, each of which is either $3$ or $6$ (but this distinction doesn't matter when we consider only the powers of $3$ .
Now we can reframe the problem again. Our method will be as follows: Suppose we choose an arbitrary pair $(i,j)$ that match the requirements, corresponding to the number of $3$ 's and the number of $5$ 's our product will have. Then how many different $h$ values for the powers of $2$ are possible?
In the $i+j$ factors we have already chosen, we obviously can't have any factors of $2$ in the $j$ factors with $5$ . However, we can have a factor of $2$ pairing with factors of $3$ , if we choose a $6$ . The maximal possible power of $2$ in these $i$ factors is thus $2^i$ , which occurs when we pick every factor to be $6$ .
We now have $n-i-j$ factors remaining, and we want to allocate these to solely powers of $2$ . For each of these factors, we can choose either a $1,2,$ or $4$ . Therefore the maximal power of $2$ achieved in these factors is when we pick $4$ for all of them, which is equivalent to $2^{2\cdot (n-i-j)}$ .
Now if we multiply this across the total $n$ factors (or $n$ dice) we have a total of $2^{2n-2i-2j} \cdot 2^i = 2^{2n-i-2j}$ , which is the maximal power of $2$ attainable in the product for a pair $(i,j)$ . Now note that every power of $2$ below this power is attainable: we can simply just take away a power of $2$ from an existing factor by dividing by $2$ . Therefore the powers of $2$ , and thus the $h$ value ranges from $h=0$ to $h=2n-i-2j$ , so there are a total of $2n+1-i-2j$ distinct values for $h$ for a given pair $(i,j)$ .
Now to find the total number of distinct triplets, we must sum this across all possible $i$ s and $j$ s. Lets take note of our restrictions on $i,j$ : the only restriction is that $i+j \leq n$ , since we're picking factors from $n$ dice.
\[\sum_{i+j\leq n}^{} 2n+1-i-2j = \sum_{i+j \leq n}^{} 2n+1 - \sum_{i+j \leq n}^{} i+2j\]
We start by calculating the first term. $2n+1$ is constant, so we just need to find out how many pairs there are such that $i+j \leq n$ . Set $i$ to $0$ : $j$ can range from $0$ to $n$ , then set $i$ to $1$ : $j$ can range from $0$ to $n-1$ , etc. The total number of pairs is thus $n+1+n+n-1+\dots+1 = \frac{(n+1)(n+2)}{2}$ . Therefore the left summation evaluates to \[\frac{(2n+1)(n+1)(n+2)}{2}\]
Now we calculate $\sum_{i+j \leq n}^{} i+2j$ . This simplifies to $\sum_{i+j \leq n}^{} i + 2 \cdot \sum_{i+j \leq n}^{} j$ . Note that because $i+j = n$ is symmetric with respect to $i,j$ , the sum of $i$ in all of the pairs will be equal to the sum of $j$ in all of the pairs. Thus this is equal to calculating $3 \cdot \sum_{i+j \leq n}^{} i$ .
In the pairs, $i=1$ appears for $j$ ranging between $0$ and $n-1$ so the sum here is $1 \cdot (n)$ . Similarly $i=2$ appears for $j$ ranging from $0$ to $n-2$ , so the sum is $2 \cdot (n-1)$ . If we continue the pattern, the sum overall is $(n)+2 \cdot (n-1) + 3 \cdot (n-2) + \dots + (n) \cdot 1$ . We can rearrange this as $((n)+(n-1)+ \dots + 1) + ((n-1)+(n-2)+ \dots + 1)+ ((n-2)+(n-3)+ \dots + 1) + \dots + 1)$
\[= \frac{(n)(n+1)}{2} + \frac{(n-1)(n)}{2}+ \dots + 1\]
We can write this in easier terms as $\sum_{k=0}^{n} \frac{(k)(k+1)}{2} = \frac{1}{2} \cdot \sum_{k=0}^{n} k^2+k$ \[=\frac{1}{2} \cdot( \sum_{k=0}^{n} k^2 + \sum_{k=0}^{n} k)\] \[= \frac{1}{2} \cdot ( \frac{(n)(n+1)(2n+1)}{6} + \frac{(n)(n+1)}{2})\] \[= \frac{1}{2} \cdot ( \frac{(n)(n+1)(2n+1)}{6} + \frac{3n(n+1)}{6}) = \frac{1}{2} \cdot \frac{n(n+1)(2n+4)}{6}\] \[= \frac{n(n+1)(n+2)}{6}\]
We multiply this by $3$ to obtain that \[\sum_{i+j \leq n}^{} i+2j = \frac{n(n+1)(n+2)}{2}\]
Thus our final answer for the number of distinct triplets $(h,i,j)$ is: \[\sum_{i+j\leq n}^{} 2n+1-i-2j = \frac{(2n+1)(n+1)(n+2)}{2} - \frac{n(n+1)(n+2)}{2}\] \[= \frac{(n+1)(n+2)}{2} \cdot (2n+1-n) = \frac{(n+1)(n+2)}{2} \cdot (n+1)\] \[= \frac{(n+1)^2(n+2)}{2}\]
Now most of the work is done. We set this equal to $936$ and prime factorize. $936 = 12 \cdot 78 = 2^3 \cdot 3^2 \cdot 13$ , so $(n+1)^2(n+2) = 936 \cdot 2 = 2^4 \cdot 3^2 \cdot 13$ . Clearly $13$ cannot be anything squared and $2^4 \cdot 3^2$ is a perfect square, so $n+2 = 13$ and $n = 11 = \boxed{A}$
~KingRavi

## Solution 2
The product can be written as \begin{align*} 2^a 3^b 4^c 5^d 6^e & = 2^{a + 2c + e} 3^{b + e} 5^d . \end{align*}
Therefore, we need to find the number of ordered tuples $\left( a + 2c + e, b+e, d \right)$ where $a$ , $b$ , $c$ , $d$ , $e$ are non-negative integers satisfying $a+b+c+d+e \leq n$ . We denote this number as $f(n)$ .
Denote by $g \left( k \right)$ the number of ordered tuples $\left( a + 2c + e, b+e \right)$ where $\left( a, b, c, e \right) \in \Delta_k$ with $\Delta_k \triangleq \left\{ (a,b,c,e) \in \Bbb Z_+^4: a+b+c+e \leq k \right\}$ .
Thus, \begin{align*} f \left( n \right) & = \sum_{d = 0}^n g \left( n - d \right) \\ & = \sum_{k = 0}^n g \left( k \right) . \end{align*}
Next, we compute $g \left( k \right)$ .
Denote $i = b + e$ . Thus, for each given $i$ , the range of $a + 2c + e$ is from 0 to $2 k - i$ . Thus, the number of $\left( a + 2c + e, b + e \right)$ is \begin{align*} g \left( k \right) & = \sum_{i=0}^k \left( 2 k - i + 1 \right) \\ & = \frac{1}{2} \left( k + 1 \right) \left( 3 k + 2 \right) . \end{align*}
Therefore, \begin{align*} f \left( n \right) & = \sum_{k = 0}^n g \left( k \right) \\ & = \sum_{k=0}^n \frac{1}{2} \left( k + 1 \right) \left( 3 k + 2 \right) \\ & = \frac{3}{2} \sum_{k=0}^n \left( k + 1 \right)^2 - \frac{1}{2} \sum_{k=0}^n \left( k + 1 \right) \\ & = \frac{3}{2} \cdot \frac{1}{6} \left( n+1 \right) \left( n+2 \right) \left( 2n + 3 \right) - \frac{1}{2} \cdot \frac{1}{2} \left( n + 1 \right) \left( n + 2 \right) \\ & = \frac{1}{2} \left( n + 1 \right)^2 \left( n + 2 \right) . \end{align*}
By solving $f \left( n \right) = 936$ , we get $n = \boxed{\textbf{(A) 11}}$ .
~Steven Chen (Professor Chen Education Palace, www.professorchenedu.com)

## Solution 3 (Cheese)
The product can be written as \begin{align*} 2^x 3^y 5^z \end{align*}
Letting $n=1$ , we get $(x,y,z)=(0,0,0),(0,0,1),(0,1,0),(1,0,0),(1,1,0),(2,0,0)$ , 6 possible values. But if the only restriction of the product if that $2x\le n,y\le n,z\le n$ , we can get $(2+1)(1+1)(1+1)=12$ possible values. We calculate the ratio \[r = \frac{\text{possible values of real situation}}{\text{possible values of ideal situation}} = \frac{6}{12}=0.5.\]
Letting $n=2$ , we get $(x,y,z)=(0,0,0),(0,0,1),(0,0,2),(0,1,0),(0,1,1),(1,0,0),(1,0,1),(1,1,0),(1,1,1),(1,2,0),$ $(2,0,0),(2,0,1),(2,1,0),(2,2,0),(3,0,0),(3,1,0),(4,0,0)$ , 17 possible values. The number of possibilities in the ideal situation is $5*3*3=45$ , making $r = 17/45 \approx 0.378$ .
Now we can predict the trend of $r$ : as $n$ increases, $r$ decreases. Letting $n=3$ , you get possible values of ideal situation= $7*4*4=112$ . $n=4$ , the number= $9*5*5=225$ . $n=5$ , the number= $11*6*6=396$ . $n=6$ , the number= $13*7*7=637,637<936$ so 6 is not the answer. $n=7$ , the number= $15*8*8=960$ . $n=8$ , the number= $17*9*9=1377$ ,but $1377*0.378$ ≈ $521$ still much smaller than 936. $n=9$ , the number= $19*10*10=1900$ ,but $1900*0.378$ ≈ $718$ still smaller than 936. $n=10$ , the number= $21*11*11=2541$ , $2541*0.378$ ≈ $960$ is a little bigger 936, but the quotient of (possible values of real situation)/(possible values of ideal situation) is much smaller than 0.378 now, so 10 is probably not the answer,so the answer is $\boxed{\textbf{(A) 11}}$ .
Check calculation: $n=11$ ,the number= $23*12*12=3312$ , $3312*0.378$ ≈ $1252$ is much bigger than 936.
~Troublemaker

## Solution 4 (Easy computation)
The key observation is if $P=2^a\cdot 3^b \cdot 5^c$ , then given $b$ and $c$ , $a$ can take any value from $0$ to $b+2d$ where $d=n-b-c$ is the number of rolls which is neither divisible by $3$ nor $5$ . We are left to calculate \[\sum_{b+c\leq n} (b+2d+1)=\sum_{b+c+d=n} (b+2d+1).\] By symmetry, $\sum_{b+c+d=n} d = \sum_{b+c+d=n} c$ . Therefore, \[\sum_{b+c\leq n}(b+2d+1)=\sum_{b+c\leq n}(b+c+d+1)=\sum_{b+c\leq n}(n+1)=(n+1)\binom{n+2}{2}.\]
The rest is the same as above.
~asops

## Solution 5 ("normalize" the product) by FireSirius
The difficulty is that a product can be formed by different combinations of 1,2,...,n. So the key thought of this solution is to set a "normalized" combination for each product.
$P=1^{k_1}\cdot 2^{k_2} \cdot 3^{k_3}\cdot 4^{k_4}\cdot 5^{k_5} \cdot 6^{k_6}$ , with $k_1+k_2+...+k_6=n$ .
For a fixed number of dice, it is easy to see that there are three basic "transformation": 1*6 = 2*3, 1*4 = 2*2, and 2*6 = 3*4, which does not change the number of dice. Other transformation like 1*6*6=3*3*4 can be viewed as a 1*6=2*3 combined with a 2*6=3*4.
So we can transform any given combination into a "normallised" combination in this way: step 1, if there are 1 and 6, then transorm them into 2*3; step 2, if there are both 1 and 4, then transform them into a 2*2; step3: if there are both 2 and 6, then transform them into 3*4. Until no more basic transformation can be made.
Now begin casework with $k_1$ :
case 1( $k_1 <= k_6$ ): all "1"s cancel with "6"s, so the product contains only 2,3,4,5,6. And now:
If "2"s are no more than remaining "6"s: all "2"s cancel with "6"s, so the "nomarlized" product consists of only $"3456"$ , with the total number of dice unchanged. No transformation can be made now and it is the same with n stars and 3 bars, so there are $C^3_{n+3}$ ways.
If "2"s are no less than remaining "6"s: all "6" cancels with "2", so the product consist of only $"2345"$ . Again, there are $C^3_{n+3}$ ways.
case 2( $k_1>=k_6$ ): all "6" cancels with "1", the remaining numbers are: 1,2,3,4,5; now if "1"s are no less than "4"s, then it can be transformed into product with only $"1235"$ ; there are, again, $C^3_{n+3}$ ways. if "1"s are no more than "4", then it is product with only 2,3,4,5, which is already counted before.
So there are three major cases: $"2345"$ , $"3456"$ and $"1235"$ , each with $C^3_{n+3}$ ways. There are overlaps: $3^{k_3} 4^{k_4} 5^{k_5}$ , which has $C^2_{n+2}$ ways, are counted in both $"2345"$ and $"3456"$ , and $2^{k_2} 3^{k_3} 5^{k_5}$ are counted in both $"2345"$ and $"1235"$ .
So, the final number is: \[3C^3_{n+3}-2C^2_{n+2}=\frac{(n+1)^2 (n+2)}{2},\] and now any possible product is counted exactly once. And then it is easily to find out $n = \boxed{\textbf{(A) 11}}$ .
~FireSirius

## Solution 6 (defining sequences)
We define:
$a_n$ is the number of possible products of the results of $n$ dice being rolled.
Now consider a modified five-sided die that excludes $5$ , having faces $1$ , $2$ , $3$ , $4$ , and $6$ . Let the number of possible products of the results of $n$ of these modified dice be equal to $b_n$ .
If in the $n$ rolls of the dice, we roll $5$ zero times, then the number of distinct products is equal to $b_n$ . If we roll $5$ once, then the number of distinct products is equal to $b_{n-1}$ . In general, if we roll $5$ $i$ times, then the number of distinct products is equal to $b_{n-i}$ . Between the different cases of how many times we roll $5$ , the products are guaranteed to be distinct. This is because in their prime factorizations, the powers of $5$ are different, and by the Fundmamental Theorem of Arithmetic, the products must be different as well.
In other words, we have found: \[a_n=\sum_{i=0}^{n} b_i\]
Now let us focus on $b_n$ , and from now on, until otherwise specified, the die will refer to the modified, 5-sided die. In these $n$ rolls of the dice, if we roll $3$ zero times and $6$ zero times, then the product must be a power of $2$ . It can range from $2^0$ to $4^n$ , which is equal to $2^{2n}$ . Therefore, there are $2n+1$ possible products. If we either roll $3$ once or $6$ once (not both), then the product must be $3$ times a power of $2$ . This power of $2$ can range from $2^0$ to $2^{2(n-1)+1}=2^{2n-1}$ , when we roll one $6$ and all other rolls are $4$ . Therefore, there are $2n$ products. In general, if we roll $3$ and $6$ a combined $i$ times, then the product must be in the form $2^k * 3^i$ , and $k$ ranges from $0$ to $2(n-i)+i=2n-i$ , resulting in $2n-i+1$ products.
In other words, we have found: \[b_n=\sum_{i=0}^{n} 2n-i+1\]
We can now calculate $b_n$ . Writing out the full sum, we get: \[b_n=(2n+1)+(2n)+\cdots+(n+1)\] This simplifies to: \[b_n=\frac{(n+1)(3n+2)}{2}=\frac{3n^2+5n+2}{2}\]
Now, finally, we can calculate $a_n$ : \[a_n=\sum_{i=0}^{n} b_i\]
\[=\sum_{i=0}^{n} \frac{3i^2+5i+2}{2}\]
\[=\sum_{i=0}^{n} \frac{3i^2}{2} + \sum_{i=0}^{n} \frac{5i}{2} + \sum_{i=0}^{n} 1\]
\[=\frac{3}{2}*\frac{n(n+1)(2n+1)}{6} + \frac{5}{2}*\frac{n(n+1)}{2} + (n+1)\]
\[=(n+1)(\frac{n(2n+1)}{4}+\frac{5n}{4}+1)\]
\[=(n+1)(\frac{2n^2+6n+4}{4})\]
\[=\frac{(n+1)^2(n+2)}{2}\]
Finally, plugging in $a_n=936$ , we get that $n=\boxed{\textbf{(A) 11}}$ .
~primenumbersfun

## Video Solution 1 by OmegaLearn
https://youtu.be/FZG1j95owTo

## Video Solution
https://youtu.be/lHtp83x1Hcw?si=DVuGnTC3hAcdmTsF
~MathProblemSolvingSkills.com

## Video Solution
https://youtu.be/BWb1dS4Jba0
~Steven Chen (Professor Chen Education Palace, www.professorchenedu.com)
### See Also
These problems are copyrighted © by the Mathematical Association of America.
These problems are copyrighted © by the Mathematical Association of America.
These problems are copyrighted © by the Mathematical Association of America.
These problems are copyrighted © by the Mathematical Association of America .