# 2019 AMC 10B Problem 25

## Problem

How many sequences of $0$ s and $1$ s of length $19$ are there that begin with a $0$ , end with a $0$ , contain no two consecutive $0$ s, and contain no three consecutive $1$ s?

$\textbf{(A) }55\qquad\textbf{(B) }60\qquad\textbf{(C) }65\qquad\textbf{(D) }70\qquad\textbf{(E) }75$

### Note

This problem is just a simplified version of 2001 AIME I, Problem 14 , and a slightly harder version of CLMC 2025 C4 .

## Solution 1 (Recursion)
Let $f(n)$ be the number of valid sequences of length $n$ (satisfying the conditions given in the problem).
We know our valid sequence must end in a $0$ . Then, since we cannot have two consecutive $0$ s, it must end in a $10$ . Now, we only have two cases: it ends with $010$ , or it ends with $110$ which is equivalent to $0110$ . Thus, our sequence must be of the forms $0\ldots010$ or $0\ldots0110$ . In the first case, the first $n-2$ digits are equivalent to a valid sequence of length $n-2$ . In the second, the first $n-3$ digits are equivalent to a valid sequence of length $n-3$ . Therefore, it must be the case that $f(n) = f(n-3) + f(n-2)$ , with $n \ge 3$ (because otherwise, the sequence would contain only 0s and this is not allowed due to the given conditions).
It is easy to find $f(3) = 1$ since the only possible valid sequence is $010$ . $f(4)=1$ since the only possible valid sequence is $0110$ . $f(5)=1$ since the only possible valid sequence is $01010$ .
The recursive sequence is then as follows:
\[f(3)=1\] \[f(4)=1\] \[f(5) = 1\] \[f(6) = 1 + 1 = 2\] \[f(7) = 1 + 1 = 2\] \[f(8) = 1 + 2 = 3\] \[f(9) = 2 + 2 = 4\] \[f(10) = 2 + 3 = 5\] \[f(11) = 3 + 4 = 7\] \[f(12) = 4 + 5 = 9\] \[f(13) = 5 + 7 = 12\] \[f(14) = 7 + 9 = 16\] \[f(15) = 9 + 12 = 21\] \[f(16) = 12 + 16 = 28\] \[f(17) = 16 + 21 = 37\] \[f(18) = 21 + 28 = 49\] \[f(19) = 28 + 37 = 65\]
So, our answer is $\boxed{\text{\bf{(C)} } 65}$ .
Contributors:
~Original Author
~solasky
~BakedPotato66
~ CrazyVideoGamez

## Solution 2 (casework)
After any particular $0$ , the next $0$ in the sequence must appear exactly $2$ or $3$ positions down the line. In this case, we start at position $1$ and end at position $19$ , i.e. we move a total of $18$ positions down the line. Therefore, we must add a series of $2$ s and $3$ s to get $18$ . There are a number of ways to do this:
Case 1 : nine $2$ s - there is only $1$ way to arrange them.
Case 2 : two $3$ s and six $2$ s - there are ${8\choose2} = 28$ ways to arrange them.
Case 3 : four $3$ s and three $2$ s - there are ${7\choose4} = 35$ ways to arrange them.
Case 4 : six $3$ s - there is only $1$ way to arrange them.
Summing the four cases gives $1+28+35+1=\boxed{\textbf{(C) }65}$ .

## Solution 3 (casework and blocks)
We can simplify the original problem into a problem where there are $2^{17}$ binary characters with zeros at the beginning and the end. Then, we know that we cannot have a block of 2 zeroes and a block of 3 ones. Thus, our only options are a block of $0$ s, $1$ s, and $11$ s. Now, we use casework:
Case 1 : Alternating 1s and 0s. There is simply 1 way to do this: $0101010101010101010$ . Now, we note that there cannot be only one block of $11$ in the entire sequence, as there must be zeroes at both ends and if we only include 1 block, of $11$ s this cannot be satisfied. This is true for all odd numbers of $11$ blocks.
Case 2 : There are 2 $11$ blocks. Using the zeroes in the sequence as dividers, we have a sample as $0110110101010101010$ . We know there are 8 places for $11$ s, which will be filled by $1$ s if the $11$ s don't fill them. This is ${8\choose2} = 28$ ways.
Case 3 : Four $11$ blocks arranged. Using the same logic as Case 2, we have ${7\choose4} = 35$ ways to arrange four $11$ blocks.
Case 4 : No single $1$ blocks, only $11$ blocks. There is simply one case for this, which is $0110110110110110110$ .
Adding these four cases, we have $1+28+35+1=\boxed{\textbf{(C) }65}$ as our final answer.
~Equinox8

## Solution 4 (similar to #3)
Any valid sequence must start with a $0$ . We can then think of constructing a sequence as adding groups of terms to this $0$ , each ending in $0$ . (This is always possible because every valid string ends in $0$ .) For example, we can represent the string $01011010110110$ as: $0-10-110-10-110-110$ . To not have any consecutive 0s, we must have at least one $1$ before the next $0$ . However, we cannot have three or more $1$ s before the next $0$ because we cannot have three consecutive $1$ s. Consequently, we can only have one or two $1$ s.
So we can have the groups: $10$ and $110$ .
After the initial $0$ , we have $18$ digits left to fill in the string. Let the number of $10$ blocks be $x$ , and $110$ be $y$ . Then $x$ and $y$ must satisfy $2x+3y=18$ . We recognize this as a Diophantine equation. Taking $\pmod{2}$ yields $y=0 \pmod{2}$ . Since $x$ and $y$ must both be nonnegative, we get the solutions $(9, 0)$ , $(6, 2)$ , $(3, 4)$ , and $(0, 6)$ . We now handle each of these cases separately.
$(9, 0)$ : Only one arrangement, namely all $10$ s.
$(6, 2)$ : We have 6 groups of $11$ , and $2$ groups of $110$ . This has $\binom{6+2}{2}=28$ cases.
$(3, 4)$ : This means we have 3 groups of $10$ , and 4 groups of $110$ . This has $\binom{3+4}{3}=35$ cases.
$(0, 6)$ : Only one arrangement, namely all $110$ .
Adding these, we have $1+28+35+1=65 \longrightarrow \boxed{(C) 65}$ . ~Math4Life2020
~edited by alpha_2 for spelling and and typos

## Solution 5 (Constructive Counting)
Suppose the number of $0$ s is $n$ . We can construct the sequence in two steps:
Step 1: put $n-1$ of $1$ s between the $0$ s;
Step 2: put the rest $19-n-(n-1)=20-2n$ of $1$ s in the $n-1$ spots where there is a $1$ . There are $\binom{n-1}{20-2n}$ ways of doing this.
Therefore the answer is \[\sum_n \binom{n-1}{20-2n} = \binom{6}{6} + \binom{7}{4} + \binom{8}{2} + \binom{9}{0} = \boxed{\textbf{(C) }65}.\]
~ asops

## Solution 6 (Recursion)
For a valid sequence of length $n$ , the sequence must be in the form of $01xx...xx10$ . By removing the $01$ at the start of the sequence and the $10$ at the end of the sequence, there are $n-4$ bits left. The $n-4$ bits left can be in the form of:
So, $f(n) = f(n-4) + 2f(n-5) + f(n-6)$
We will calculate $f(19)$ by Dynamic Programming .
$f(3) = 1$
$f(4) = 1$
$f(5) = 1$
$f(6) = 2$
$f(7) = 2$
$f(8) = 3$
$f(9) = f(5) + 2 \cdot f(4) + f(3) = 1 + 2 \cdot 1 + 1 = 4$
$f(10) = f(6) + 2 \cdot f(5) + f(4) = 2 + 2 \cdot 1 + 1 = 5$
$f(11) = f(7) + 2 \cdot f(6) + f(5) = 2 + 2 \cdot 1 + 1 = 7$
$f(12) = f(8) + 2 \cdot f(7) + f(6) = 3 + 2 \cdot 2 + 2 = 9$
$f(13) = f(9) + 2 \cdot f(8) + f(7) = 4 + 2 \cdot 3 + 2 = 12$
$f(14) = f(10) + 2 \cdot f(9) + f(8) = 5 + 2 \cdot 4 + 3 = 16$
$f(15) = f(11) + 2 \cdot f(10) + f(9) = 7 + 2 \cdot 5 + 4 = 21$
$f(16) = f(12) + 2 \cdot f(11) + f(10) = 9 + 2 \cdot 7 + 5 = 28$
$f(17) = f(13) + 2 \cdot f(12) + f(11) = 12 + 2 \cdot 9 + 7 = 37$
$f(18) = f(14) + 2 \cdot f(13) + f(12) = 16 + 2 \cdot 12 + 9 = 49$
$f(19) = f(15) + 2 \cdot f(14) + f(13) = 21 + 2 \cdot 16 + 12 = \boxed{\text{\bf{(C)} } 65}$
We can further prove $f(n) = f(n-4) + 2f(n-5) + f(n-6)$ is equivalent to $f(n) = f(n-2) + f(n-3)$
Let $k(n) = f(n-2) + f(n-3)$
$k(n-2) = f(n-4) + f(n-5)$
$k(n-3) = f(n-5) + f(n-6)$
$k(n-2)+ k(n-3) = f(n-4) + 2f(n-5) + f(n-6) = f(n)$
$f(n) = k(n-2)+ k(n-3)$
$f(n-2) = k(n-4)+ k(n-5)$
$f(n-3) = k(n-5)+ k(n-6)$
$k(n) = f(n-2) + f(n-3) = k(n-4)+ k(n-5) + k(n-5)+ k(n-6) = k(n-4) + 2k(n-5) + k(n-6)$
So $k(n)$ is the same as $f(n)$ .
~ isabelchen

## Solution 7 (Quick Solution by Estimating)
Using the tree diagram, you quickly notice that your answer must be very close to a power of $2$ due to the splitting of the tree branches in a tree diagram. $2^6$ is $64$ , which is very close to $65$ , thus giving our answer of $\boxed{\textbf{(C) }65}$ .
~MichaeLLin16 ~Minor Edit and Moving by HappySharks

## Solution 8 (Sequence Dividing and Path Counting)
You can split the sequence into $0$ and $6$ strings of three numbers, which can only be $010$ , $011$ , $110$ , $101$ , labelled as A,B,C,D respectively. For example, $0101....010$ is labelled $0DADADA$ . This can also be stated as 0, $D_{1}, A_{2}, D_{3},$ etc. The problem is equivalent to find the number of such sequences. For each string, A can be followed by C and D, B can be followed by A and B, C can be followed by C and D, D can be followed by A,B, and D. If we define $n(A_{i})$ as number of possible sequences that ends with string A at the $i$ th spot (thus be $3i+1$ numbers long), we may find relationship between these numbers by noting that, for the $i+1$ th string, with $i \geq 1$
Since the first number of the sequence must be zero, we must start with $n(A_1) = n(B_1) = 0, n(C_1) = n(D_1) = 1$ . Using the above steps to evolve the situation from i = 1 to i = 6, we get $n(A_{6}) = 37, n(B_{6}) = 37, n(C_{6}) = 28, n(D_{6}) = 49$ . Since the sequence ends with 0, we only need to sum $n(A_{6})$ and $n(C_{6})$ , which yields $37+28=65$ . $\boxed{\textbf{(C) }65}$
Solution by ~Cc2010cc2015
minor edit by ~CLA

## Solution 9
We define a sequences of $01$ ( $a$ ) or $011$ ( $b$ ). Observe that we can put the the $a$ 's and $b$ 's in any way and we meet all the different requirements. Note that this can be found through just playing around with the problem's mechanics. Now we can see a big problem. With sequences of $a$ and $b$ , the main sequence always end with a $1$ . '
Now a simple fix is just to add zero to the end of the sequence, shortening it effectively to 18 undecided digits. Now we have multiple cases.
\begin{align*} 18 &= 9a + 0b &\rightarrow \dfrac{(9+0)!}{9!} \\ &= 6a + 2b &\rightarrow \dfrac{(6+2)!}{6!}\\ &= 3a + 4b &\rightarrow \dfrac{(3 + 4)!}{4!}\\ &= 0a + 6b &\rightarrow \dfrac{(0+6)!}{6!}\\ \end{align*}
(Here's how I was able to see this, I put a zero, than I have to put a one, and then I can put a one or a zero. Then I saw that after every zero, a certain pattern repeats.)
- Created by wiselion :)

## Solution 10 (Recursion)
Lets use recursion to solve this problem. First, lets try out making this problem smaller by replace $19$ with $1,2,$ and $3$ . Let $a_n$ be the number of ways to create strings of $0$ 's and $1$ 's that follow the restrictions. So, $a_1=1$ because the only possibility is just $0$ . We also have $a_2=0$ since it must start with $0$ and end with $0$ but there can not be two consecutive $0$ 's. Lastly, $a_3=1$ (just $010$ ). Now, we can find the recurrence equation. Lets start with a string of length $n$ . We know it must go something like \[0 \_\_\_\ldots\_\_\_ 0\] . We can start filling in some of this. It could go like \[0 1 0 \_\ldots\_\_\_ 0\] or \[0 1 1 \_\ldots\_\_\_ 0\] . Now, lets examine these closely. In the first case, this is basically just $a_{n-2}$ because the length of the string is now only $n-2$ . Similarly with the second case, it is just $a_{n-3}$ . So, we can write the equation $a_n=a_{n-2}+a_{n-3}$ . Now, we simply continuously plug in small values of $n$ , and keep increasing them to get to $19$ . So, we keep continuously plugging in values of $n$ to get new values of $n$ to give us an answer of $a_{19}=\boxed{\text{\bf{(C)} } 65}$ .
-jb2015007

## Video Solution by OmegaLearn
https://youtu.be/WpSpnx8PPnc?t=94
~pi_is_3.14

## Video Solution 1
https://youtu.be/VamT49PjmdI

## Video Solution 2
https://www.youtube.com/watch?v=eMWV87zmPFs&
~avibatra
### See Also
These problems are copyrighted © by the Mathematical Association of America.
These problems are copyrighted © by the Mathematical Association of America.
These problems are copyrighted © by the Mathematical Association of America.
These problems are copyrighted © by the Mathematical Association of America .