# 2006 AMC 10B Problem 1

## Problem

What is $(-1)^{1} + (-1)^{2} + ... + (-1)^{2006}$ ?

$\textbf{(A)} -2006\qquad \textbf{(B)} -1\qquad \textbf{(C) } 0\qquad \textbf{(D) } 1\qquad \textbf{(E) } 2006$

## Solution 1
Since $-1$ raised to an odd integer is $-1$ and $-1$ raised to an even integer exponent is $1$ :
$(-1)^{1} + (-1)^{2} + ... + (-1)^{2006} = (-1) + (1) + ... + (-1)+(1) = \boxed{\textbf{(C) }0}.$

## Solution 2
The Using the formula for the first $n$ terms of a geometric series, with $n = 2006$ , $a = (-1)^{1} = -1$ , and $r = -1$ , the sum can also be obtained:
$\frac{a(1-r^n)}{1-r} = \frac{-1(1 - (-1)^{2006})}{1 + 1} = \frac{-1(1 - 1)}{2} = \frac{0}{2} = \boxed{\textbf{(C) }0}$
~anabel.disher
### See Also
These problems are copyrighted © by the Mathematical Association of America.
These problems are copyrighted © by the Mathematical Association of America.
These problems are copyrighted © by the Mathematical Association of America.
These problems are copyrighted © by the Mathematical Association of America .