# 2003 AMC 10A Problem 18

## Problem

What is the sum of the reciprocals of the roots of the equation $\frac{2003}{2004}x+1+\frac{1}{x}=0$ ?

$\mathrm{(A) \ } -\frac{2004}{2003}\qquad \mathrm{(B) \ } -1\qquad \mathrm{(C) \ } \frac{2003}{2004}\qquad \mathrm{(D) \ } 1\qquad \mathrm{(E) \ } \frac{2004}{2003}$

## Solution 1
Multiplying both sides by $x$ :
$\frac{2003}{2004}x^{2}+x+1=0$
Let the roots be $a$ and $b$ .
The problem is asking for $\frac{1}{a}+\frac{1}{b}= \frac{a+b}{ab}$
By Vieta's Formulas :
$a+b=(-1)^{1}\frac{1}{\frac{2003}{2004}}=-\frac{2004}{2003}$
$ab=(-1)^{2}\frac{1}{\frac{2003}{2004}}=\frac{2004}{2003}$
So the answer is $\frac{a+b}{ab}=\frac{-\frac{2004}{2003}}{\frac{2004}{2003}}=-1 \Rightarrow\boxed{\mathrm{(B)}\ -1}$ .

## Solution 2
Dividing both sides by $x$ ,
$\frac{2003}{2004}+\frac 1x+\frac{1}{x^2}=0$ ,
we see by Vieta's Formulas that the sum of the roots is $-1 \Rightarrow\boxed{\mathrm{(B)}\ -1}$ .

## Solution 3(Alternate Approach to Solution 1)
Re-stating and multiplying $\frac{1}{x}$ by $\frac{2004}{2004}$ , we have $\frac{2003x}{2004} + \frac{2004}{2004x} + 1 = 0$ .
Simplifying, we have $\frac{2003}{2004}+\frac{\frac{2004}{x}}{2004}=-1.$
Putting this together, we have $\frac{2003+\frac{2004}{x}}{2004}=-1.$
Simplifying, we have $2004x + \frac{2004}{x} = -2004.$
Multiplying both sides by $x,$ we have $2003x^2+2004=-2004x.$
Moving $-2004x$ to the left side, we have $2003x^2 + 2004x + 2004 = 0.$
Let's go back and see what we want.
We want the sum of the reciprocals of the roots, in which if the roots were to be called $r_1$ and $r_2,$ we would want $\frac{1}{r_1}+\frac{1}{r_2}=\frac{r_1 + r_2}{r_1 \cdot r_2}$ .
We can use Vieta's Formulas to solve the sum of the roots and the product of the roots.
We have that the sum of the two roots is $\frac{-b}{a}$ where the quadratic is $ax^2+bx+c=0.$
In this case, $a=2003$ and $b=2004$ .
Therefore, $r_1+r_2=-\frac{2004}{2003}.$
We have that the product of the two roots is $\frac{c}{a}$ where the quadratic is $ax^2+bx+c=0.$
In this case, $c=2004$ and $a=2003.$
Therefore, $r_1 \cdot r_2 = \frac{2004}{2003}.$
Now that we have the sum and product of the roots, we can substitute back into the expression of what we want.
We have $\frac{-\frac{2004}{2003}}{\frac{2004}{2003}}=-\frac{2004}{2003} \cdot \frac{2003}{2004} = \boxed{\mathrm{(B)}\ -1}.$
~mathboy282

## Video Solution
https://youtu.be/3dfbWzOfJAI?t=456
~ pi_is_3.14

## Video Solution
https://youtu.be/j1nVw3ASBYU
~savannahsolver
### See Also
These problems are copyrighted © by the Mathematical Association of America.
These problems are copyrighted © by the Mathematical Association of America.
These problems are copyrighted © by the Mathematical Association of America.
These problems are copyrighted © by the Mathematical Association of America .