# 2025 AMC 12B Problem 10

## Problem

The altitude to the hypotenuse of a $30^\circ{-}60^\circ{-}90^\circ$ is divided into two segments of lengths $x<y$ by the median to the shortest side of the triangle. What is the ratio $\tfrac{x}{x+y}$ ?

$\textbf{(A) } \dfrac{3}{7} \qquad \textbf{(B) } \dfrac{\sqrt3}{4} \qquad \textbf{(C) } \dfrac{4}{9} \qquad \textbf{(D) } \dfrac{5}{11} \qquad \textbf{(E) } \dfrac{4\sqrt3}{15}$

### Diagram

[asy] /* Made by MRENTHUSIASM */ size(250); pair A, B, C, D, E, F; A = (0,1); B = origin; C = (sqrt(3),0); D = foot(B,A,C); E = midpoint(A--B); F = intersectionpoint(B--D,C--E); markscalefactor=0.008; draw(rightanglemark(A,B,C)^^rightanglemark(B,D,C),red+linewidth(1.25)); draw(A--B--C--cycle,linewidth(1.25)); draw(B--D^^C--E,linewidth(1.25)); add(pathticks(A--E, 1, .5, 0, 10, red+linewidth(1.25))); add(pathticks(E--B, 1, .5, 0, 10, red+linewidth(1.25))); label("$x$",midpoint(D--F),1.25*dir(-45),red); label("$y$",midpoint(F--B),1.5*dir(-10),red); label("$30^{\circ}$",C,7*dir(165),red); label("$60^{\circ}$",A,4*dir(-63),red); [/asy] ~MRENTHUSIASM

## Solution 1 (Mass Points)
Without loss of generality, let $\triangle ABC$ have side-lengths $AB=2, BC=2\sqrt{3},$ and $AC=4.$ Let $D$ be the foot of the perpendicular from $B$ to $\overline{AC}, \ E$ be the midpoint of $\overline{AB},$ and $F$ be the intersection of $\overline{CE}$ and $\overline{BD}.$ Note that $\triangle ADB$ and $\triangle BDC$ are both $30^\circ{-}60^\circ{-}90^\circ$ triangles. From the side-length ratio, we get $AD=1$ and $DC=3.$
We obtain the following diagram: [asy] /* Made by MRENTHUSIASM */ size(250); pair A, B, C, D, E, F; A = (0,1); B = origin; C = (sqrt(3),0); D = foot(B,A,C); E = midpoint(A--B); F = intersectionpoint(B--D,C--E); markscalefactor=0.008; draw(rightanglemark(A,B,C)^^rightanglemark(B,D,C),red+linewidth(1.25)); draw(A--B--C--cycle,linewidth(1.25)); draw(B--D^^C--E,linewidth(1.25)); label("$1$",midpoint(A--E),1.5*W,red); label("$1$",midpoint(E--B),1.5*W,red); label("$2\sqrt{3}$",midpoint(B--C),1.5*S,red); label("$x$",midpoint(D--F),1.25*dir(-45),red); label("$y$",midpoint(F--B),1.5*dir(-10),red); label("$30^{\circ}$",C,7*dir(165),red); label("$60^{\circ}$",A,4*dir(-63),red); label("$1$",midpoint(A--D),1.5*midpoint(A--D),red); label("$3$",midpoint(D--C),1.5*dir(70),red); label("$A$",A,1.5*NW); label("$B$",B,1.5*SW); label("$C$",C,1.5*SE); label("$D$",D,1.5*NE); label("$E$",E,1.5*W); label("$F$",F,2*dir(-75)); [/asy] From here, we will proceed with mass points . Throughout this solution, we will use $W_P$ to denote the weight of point $P.$
Let $W_C=1.$ Since $3AD=DC,$ it follows that $W_A=3$ and $W_D=W_C+W_A=4.$ Since $AE=EB$ and $W_A=3,$ it follows that $W_B=3.$
Now we focus on $\overline{BD}:$ Since $W_B=3$ and $W_D=4,$ we have $\frac{DF}{FB}=\frac xy=\frac34.$ Therefore, the answer is \[\frac{x}{x+y}=\frac{3}{3+4}=\boxed{\textbf{(A) } \dfrac{3}{7}}.\]
~lprado
~MRENTHUSIASM

## Solution 2 (Similar Triangles)
This solution refers to the diagram in Solution 1, with the definitions slightly modified.
Let $AB=2$ . Label the foot of the median $M$ and the foot of the altitude $H$ . In $\triangle ABH$ , we construct the midsegment $\overline{MP}$ , which is parallel to $\overline{BH}$ and half as long as $\overline{BH}$ . In addition, let $F$ be the intersection of $\overline{CM}$ and $\overline{BH}$ .
We obtain the following diagram: [asy] /* Made by MRENTHUSIASM */ size(250); pair A, B, C, H, M, F, P; A = (0,1); B = origin; C = (sqrt(3),0); H = foot(B,A,C); M = midpoint(A--B); F = intersectionpoint(B--H,C--M); P = midpoint(A--H); markscalefactor=0.008; draw(rightanglemark(A,B,C)^^rightanglemark(B,H,C),red+linewidth(1.25)); draw(A--B--C--cycle,linewidth(1.25)); draw(B--H^^C--M,linewidth(1.25)); draw(M--P,dashed+linewidth(1.25)); label("$1$",midpoint(A--M),1.5*W,red); label("$1$",midpoint(M--B),1.5*W,red); label("$2\sqrt{3}$",midpoint(B--C),1.5*S,red); label("$x$",midpoint(H--F),1.25*dir(-45),red); label("$y$",midpoint(F--B),1.5*dir(-10),red); label("$30^{\circ}$",C,7*dir(165),red); label("$60^{\circ}$",A,4*dir(-63),red); label("$\frac{1}{2}$",midpoint(A--P),1.5*midpoint(A--P),red); label("$\frac{1}{2}$",midpoint(P--H),1.5*midpoint(H--H),red); label("$3$",midpoint(H--C),1.5*dir(70),red); label("$A$",A,1.5*NW); label("$B$",B,1.5*SW); label("$C$",C,1.5*SE); label("$H$",H,1.5*NE); label("$M$",M,1.5*W); label("$P$",P,1.5*NE); label("$F$",F,2*dir(-75)); [/asy]
We can calculate that $PH=\frac{1}{2}$ and $HC=3$ By similar triangles $\triangle HFC \sim \triangle PMC$ , we have $\frac{x}{PM}=\frac{HC}{PC}=\frac{3}{3+\frac{1}{2}}=\frac{6}{7}$ . Also by similar triangles $\triangle PMA \sim \triangle HBA$ , we have $\frac{PM}{x+y}=\frac{1}{2}$ . Combining these, we get $\frac{x}{x+y}=\boxed{\textbf{(A) } \dfrac{3}{7}}$ .
Note: Thanks MRENTHUSIASM for original diagram.
~gimmeaworkingusername

## Solution 3 (Similar Triangles)
This solution refers to the definitions and the diagram in Solution 1.
Let $M$ be the midpoint of $\overline{AC},$ so $DM=1.$ Let $G$ be the intersection of $\overline{BM}$ and $\overline{CE},$ so $G$ is the centroid of $\triangle ABC.$ In addition, we construct $\overline{DE},$ as shown below: [asy] /* Made by MRENTHUSIASM */ size(250); pair A, B, C, D, E, F, M, G; A = (0,1); B = origin; C = (sqrt(3),0); D = foot(B,A,C); E = midpoint(A--B); F = intersectionpoint(B--D,C--E); M = midpoint(A--C); G = centroid(A,B,C); markscalefactor=0.008; draw(rightanglemark(A,B,C)^^rightanglemark(B,D,C),red+linewidth(1.25)); draw(A--B--C--cycle,linewidth(1.25)); draw(B--D^^C--E,linewidth(1.25)); draw(E--D^^B--M,dashed+linewidth(1.25)); label("$1$",midpoint(A--E),1.5*W,red); label("$1$",midpoint(E--B),1.5*W,red); label("$2\sqrt{3}$",midpoint(B--C),1.5*S,red); label("$x$",midpoint(D--F),1.25*dir(-45),red); label("$y$",midpoint(F--B),1.5*dir(-10),red); label("$30^{\circ}$",C,7*dir(165),red); label("$60^{\circ}$",A,4*dir(-63),red); label("$1$",midpoint(A--D),1.5*midpoint(A--D),red); label("$1$",midpoint(D--M),1.5*midpoint(D--M),red); label("$A$",A,1.5*NW); label("$B$",B,1.5*SW); label("$C$",C,1.5*SE); label("$D$",D,1.5*D); label("$E$",E,1.5*W); label("$F$",F,2*dir(-75)); label("$M$",M,1.5*M); label("$G$",G,1.5*S); [/asy] In any right triangle, since the median to the hypotenuse is half as long as the hypotenuse, we get $BM=\frac{1}{2}AC=2.$ Moreover, in any triangle, since the centroid divides each median into parts in the ratio $2:1,$ with the centroid being twice as close to the midpoint of a side as it is to the opposite vertex, we get $BG=\frac43$ and $GM=\frac23.$
Note that $\triangle ABM$ is an equilateral triangle with side-length $2.$ By the SAS similarity, we have $\triangle ABM \sim \triangle AED.$ Therefore, we conclude that $ED=1$ and $\overline{ED}\parallel\overline{BM}.$
By the AA Similarity, we have $\triangle DEF \sim \triangle BGF,$ from which $\frac xy = \frac{1}{4/3} = \frac34.$ It follows that \[\frac{x}{x+y}=\frac{3}{3+4}=\boxed{\textbf{(A) } \dfrac{3}{7}}.\] ~MRENTHUSIASM

## Solution 4 (Similar Triangles)
This solution refers to the definitions and the diagram in Solution 1.
Since $E$ is the midpoint of $\overline{AB}$ , we have $AE=1$ , and because $\angle A=60^\circ$ and $AD=1$ , $\triangle AED$ is equilateral. Its perpendicular bisector meets $\overline{AE}$ at $H$ , giving $AH=HE=\tfrac12$ and $DH=\tfrac{\sqrt3}{2}$ .
Extend $\overline{CE}$ past $E$ to $G$ so that $\overline{GD}$ is parallel to $\overline{BC}$ and is the perpendicular bisector of $\overline{AE}$ , so $H$ lies on both $\overline{GD}$ and $\overline{AE}$ :
[asy] size(325); pair A, B, C, D, E, F, G, H; A = (0,2); B = origin; C = (2*sqrt(3),0); D = foot(B,A,C); E = midpoint(A--B); F = intersectionpoint(B--D,C--E); // G and H for the parallel/perpendicular construction G = (-sqrt(3), 1.5); H = (0, 1.5); markscalefactor=0.015; // Draw figure draw(rightanglemark(A,B,C)^^rightanglemark(B,D,C),red+linewidth(1.25)); draw(A--B--C--cycle,linewidth(1.25)); draw(B--D,linewidth(1.25)); draw(C--E,linewidth(1.25)); draw(A--E,linewidth(1.25)); draw(E--G,dashed+linewidth(1.25)); draw(G--D,dashed+linewidth(1.25)); draw(E--D,dashed+linewidth(1.25)); // equal tick marks add(pathticks(A--E, 1, .5, 0, 12, red+linewidth(1.25))); add(pathticks(E--B, 1, .5, 0, 12, red+linewidth(1.25))); // labels label("$x$",midpoint(D--F),1.25*dir(-45),red); label("$y$",midpoint(F--B),1.5*dir(-10),red); label("$30^{\circ}$",C,7*dir(165),red); label("$60^{\circ}$",A,4*dir(-63),red); label("$1$",midpoint(E--B),2.5*W,red); label("$2\sqrt{3}$",midpoint(B--C),1.5*S,red); label("$1$",midpoint(A--D),1.5*midpoint(A--D),red); label("$3$",midpoint(D--C),1.5*dir(70),red); // Point labels label("$A$",A,1.5*NW); label("$B$",B,1.5*SW); label("$C$",C,1.5*SE); label("$D$",D,1.5*NE); label("$E$",E,1.5*W); label("$F$",F,2*dir(-75)); label("$G$",G,1.5*NW); label("$H$",H,1.5*dir(135)); [/asy]
By AA similarity, $\triangle BCE \sim \triangle HGE$ because $\angle BEC=\angle HEG$ and $\angle BCE=\angle HGE$ ( $GD\parallel BC$ ). Thus $\frac{GH}{BC}=\frac{HE}{BE}$ , and with $HE=\tfrac{1}{2}$ , $BE=1$ , and $BC=2\sqrt3$ , we get $\frac{GH}{2\sqrt3}=\frac{\frac{1}{2}}{1}$ so $GH=\sqrt3$ .
Also by AA similarity, $\triangle BCF \sim \triangle DGF$ because $\angle BFC=\angle DFG$ and $\angle BCF=\angle DGF$ ( $GD\parallel BC$ ). Therefore $\frac{DF}{BF}=\frac{DG}{BC}$ . Since $DG=DH+HG=\frac{\sqrt3}{2}+\sqrt3=\frac{3\sqrt3}{2}$ and $BC=2\sqrt3$ , we obtain $\frac{DF}{BF}=\frac{x}{y}=\frac{\frac{3\sqrt3}{2}}{2\sqrt3}=\frac{3}{4}$ , so $y=\frac43x$ .
Finally, $\frac{x}{x+y}=\frac{x}{x+\frac{4}{3}x}=\frac{x}{\frac{7}{3}x}=\boxed{\textbf{(A) } \dfrac{3}{7}}$ .
~Gymnastics15 (Mikenever Dai)
~MRENTHUSIASM (Original Diagram)

## Solution 5 (Similar Triangles)
This solution refers to the definitions in Solution 1.
Draw a line perpendicular to $BC$ from $D$ , intersecting $BC$ at $G$ , and intersecting $CE$ at $H$ . Let $a = AE$ . We know that $\triangle DHF \sim \triangle BEF$ by AA. We also know that $AE = EB = DA$ . We find that $BG = \frac{a\sqrt{3}}{2}$ , and $GC = BC - BG = 2a\sqrt{3} - \frac{a\sqrt{3}}{2} = \frac{3a\sqrt{3}}{2}$ . Because $\triangle CHG \sim \triangle CEB$ , $HG = \frac{a}{2a\sqrt{3}} \cdot \frac{3a\sqrt{3}}{2} = \frac{3}{4}a$ , and $DG = \frac{3}{2}a$ due to 30-60-90 triangle properties, $DH = \frac{3}{4}a$ . Because $\triangle DHF \sim \triangle BEF$ , $\frac{DH}{EB} = \frac{DF}{FB}$ , $\frac{\frac{3a}{4}}{a} = \frac{3}{4} = \frac{DF}{FB}$ , and $\frac{DF}{DB}=\boxed{\textbf{(A) } \dfrac{3}{7}}$ .
(You can tell $DF$ is shorter than $FB$ visually)
~shaodavin
~penguin_pro (Solution Format Change)

## Solution 6 (Coordinates)
WLOG, let the triangle have hypotenuse $12$ . Situate it in the coordinate plane such the A is at $(0,0)$ , B is at $(6,0)$ , and C is at $(6,6\sqrt{3})$ .
Let $h$ be the altitude from $A$ to $BC$ . From the area formula we get $1/2 \cdot 6\cdot6\sqrt{3} =1/2\cdot12\cdot h$
$h = 3\sqrt{3}$
The shortest side is $AB$ with side length $6$ , so the median from $C$ to $AB$ will be at $(3,0)$ . Finding the equation of the line through that point to C, find that the slope is $\frac{6\sqrt{3}-0}{6-3}=2\sqrt3$ . Plugging the point $(3,0)$ into $y=2\sqrt{3}x+b$ , we get that $0=6\sqrt{3}+b$ , which simplifies to $b=-6\sqrt{3}$ So, the equation of the line of the median from $C$ is $y=2\sqrt{3}x-6\sqrt3$
The line of the altitude from $B$ to the hypotenuse is perpendicular to the line of the hypotenuse which has slope $6\sqrt{3}/6=\sqrt{3}$
So, the altitude line has slope $\frac{-1}{\sqrt{3}}=-\frac{\sqrt{3}}{3}$ , and the line passes through the point $B = (6,0)$ Solving for the equation using similar methods above, we get $y=-\frac{\sqrt{3}}{3}x+2\sqrt{3}$
Using the two equations and solving for their intersection, we get $y=2\sqrt{3}x-6\sqrt3=-\frac{\sqrt{3}}{3}x+2\sqrt{3}$ , which simplifies to $8\sqrt3=\frac{7\sqrt{3}}{3}x$ , so $x=24/7$ Using this $x$ value, we get $y=2\sqrt{3}\cdot24/7-6\sqrt{3}=6\sqrt{3}/7$
Finding the distance from this intersection to B, $d=\sqrt{(6-24/7)^2+(0-6\sqrt{3}/7)^2} = \sqrt{324/49+108/49}=\frac{12\sqrt{3}}{7}$
This is greater than half of the calculated altitude value from above ( $3\sqrt{3}$ ), so the shorter side length is $3\sqrt{3}-\frac{12\sqrt{3}}{7}=\frac{9\sqrt{3}}{7}$
Lastly, taking the ratio of the lengths, $\frac{\frac{9\sqrt{3}}{7}}{3\sqrt{3}}=\frac{9}{21}=\boxed{\textbf{(A) } \dfrac{3}{7}}$
-Failure.net (minor edits and latex edits by Wen_Liang)

## Solution 7 (Symmedian and Bary)
Notice that the smaller right triangle with the original $30^\circ$ angle can be obtained with a dilation and a reflection over the original triangle’s angle bisector. Hence it is not too hard to see that the original median is a symmedian to this smaller triangle. Recall that the barycentric equation for the symmedian is in the form $\frac x{a^2}=\frac y{b^2}$ , and we have $a,b=\sqrt3,2$ in a $30^\circ-60^\circ-90^\circ$ triangle. Hence $x:y=4:3$ and we get the ratio $\textbf{(A) } \dfrac{3}{7}$ , or A relatively quickly.
~benjamintontungtungtungsahur

## Solution 8 (Trigonometry Bash)
Let the triangle be called $\triangle ABC$ , with $\angle C=90^{\circ}$ and $\angle A=30^{\circ}$ . Then let the altitude from $C$ intersect with $AB$ at a point $D$ , and the median from $A$ intersect $BC$ at the point $E$ . WLOG, let $AB=2$ , $AC=\sqrt{3}$ , and $BC=1$ . Then $BE=EC=\frac12$ , and by similar triangles, $DBC$ is also $30^{\circ}-60^{\circ}-90^{\circ}$ , and so $DB=\frac12$ and hence $AD=\frac32$ . Therefore, $DC=\sqrt{3}\cdot\frac12=\frac{\sqrt{3}}2$ . Also, we have that $\tan(\angle EAC)=\frac1{2\sqrt{3}}\implies\angle EAC=\arctan\left(\frac1{2\sqrt{3}}\right)$ . Hence, $\angle BAE=30^{\circ}-\arctan\left(\frac1{2\sqrt{3}}\right)$ . Now we can set up to solve for $x$ ; we have that $\tan(\angle BAE)=\frac{x}{\frac32}$ . $\tan(\angle BAE)=\frac{\frac1{\sqrt{3}}-\frac1{2\sqrt{3}}}{1+\frac1{\sqrt{3}}\cdot\frac1{2\sqrt{3}}}=\frac{\frac1{2\sqrt{3}}}{\frac76}=\frac1{2\sqrt{3}}\cdot\frac67=\frac{\sqrt{3}}7$ . Hence $x=\frac32\cdot\frac{\sqrt{3}}7=\frac{3\sqrt{3}}{14}$ , and therefore since we found earlier that $x+y=DC=\frac{\sqrt{3}}2$ , we have that $\frac{x}{x+y}=\frac{\frac{3\sqrt{3}}{14}}{\frac{\sqrt{3}}2}=\boxed{\textbf{(A) } \dfrac{3}{7}}$ .
~singularity1

## Solution 9 (Easier to Understand, Using Similar 30-60-90 Triangles)
Let the triangle be $\triangle ABC$ , where $\angle A=30^\circ$ , $\angle B=60^\circ$ , and $\angle C=90^\circ$ . Let the point where the altitude of $AB$ and $AB$ intersect be $G$ . Let the intersection between the median of $CB$ and the altitude of $AB$ be $E$ . $x=EG$ and $y=CE$ .
Draw a segment, $DF$ , so that it is perpendicular to $AC$ and passes through $E$ . This creates two small $30^\circ{-}60^\circ{-}90^\circ$ triangles, $\triangle ECD$ and $\triangle EFG$ . Using the Side-Splitter Thm., we know that $DE=EF$ . Let $DE=EF=2$ . Using the rules of $30^\circ{-}60^\circ{-}90^\circ$ triangles, we can find that $x=EG=\frac{2}{2}\cdot\sqrt{3}=\sqrt{3}$ and that $y=CE=\frac{2}{\sqrt{3}}\cdot2=\frac{4}{\sqrt{3}}=\frac{4\sqrt{3}}{3}$ . Therefore, \[\frac{x}{x+y}=\frac{\sqrt{3}}{\sqrt{3}+\frac{4\sqrt{3}}{3}}=\frac{\sqrt{3}}{\frac{3\sqrt{3}}{3}+\frac{4\sqrt{3}}{3}}=\frac{\sqrt{3}}{\frac{7\sqrt{3}}{3}}=\sqrt{3}\cdot\frac{3}{7\sqrt{3}}=\frac{3\sqrt{3}}{7\sqrt{3}}=\boxed{\textbf{(A) } \dfrac{3}{7}}.\]
~Bittle

## Solution 10 (Ruler)
Since rulers are allowed on the AMC 10, we can draw out the figure accurately with a ruler. Draw a $30-60-90$ triangle at any scale that you want (I used $1$ inch, $\sqrt{3}$ inches, and $2$ inches for my sides), then draw the altitude to the hypotenuse and the median to the shortest side on the triangle. Find the ratio of the short part of the altitude divided by the median and the total length of the altitude. Assuming that you drew accurately, the answer is then $\boxed{\textbf{(A) } \dfrac{3}{7}}$ .
~mathcantcount1plus1is3

## Solution 11 (Law of Cosines Bash)
[asy] unitsize(0.3mm); /* Generated by Cloud's Excalidraw to Asymptote */ draw((-561, -520)--(-553, -515)--(-548, -523)--(-556, -528)--cycle, rgb(0.94, 0.54, 0)+linewidth(1)+solid);draw((-700, -590)--(-691, -590)--(-691, -599)--(-700, -599)--cycle, rgb(0.94, 0.54, 0)+linewidth(1)+solid);draw((-567, -510)--(-559, -505)--(-554, -513)--(-562, -518)--cycle, rgb(0.94, 0.54, 0)+linewidth(1)+solid);draw((-701, -260)--(-701, -600)--(-501, -600)--(-701, -260), rgb(0.11, 0.11, 0.11)+linewidth(2)+solid); draw((-701, -260)--(-601, -600), rgb(0.11, 0.11, 0.11)+linewidth(2)+solid); draw((-701, -600)--(-553, -515), rgb(0.11, 0.11, 0.11)+linewidth(2)+solid); draw((-648, -594)--(-648, -606), rgb(0.94, 0.54, 0)+linewidth(2)+solid); draw((-553, -594)--(-553, -606), rgb(0.94, 0.54, 0)+linewidth(2)+solid); draw((-602, -600)--(-552, -515), rgb(0.11, 0.11, 0.11)+linewidth(2)+solid); filldraw(shift(-701, -601) * rotate(0) * ellipse((0, 0), 4, 4), rgb(0.11, 0.11, 0.11), rgb(0, 0, 0)+linewidth(0)+solid); filldraw(shift(-601, -601) * rotate(0) * ellipse((0, 0), 4, 4), rgb(0.11, 0.11, 0.11), rgb(0, 0, 0)+linewidth(0)+solid); filldraw(shift(-502, -600) * rotate(0) * ellipse((0, 0), 4, 4), rgb(0.11, 0.11, 0.11), rgb(0, 0, 0)+linewidth(0)+solid); filldraw(shift(-701, -262) * rotate(0) * ellipse((0, 0), 4, 4), rgb(0.11, 0.11, 0.11), rgb(0, 0, 0)+linewidth(0)+solid); filldraw(shift(-552, -515) * rotate(0) * ellipse((0, 0), 4, 4), rgb(0.11, 0.11, 0.11), rgb(0, 0, 0)+linewidth(0)+solid); filldraw(shift(-616, -551) * rotate(0) * ellipse((0, 0), 4, 4), rgb(0.11, 0.11, 0.11), rgb(0, 0, 0)+linewidth(0)+solid); draw((-519, -598)--(-517, -590)--(-511, -586), rgb(0.87, 0.19, 0.19)+linewidth(2)+solid); draw((-699, -582)--(-691, -584)--(-687, -590), rgb(0.87, 0.19, 0.19)+linewidth(2)+solid); draw((-545, -530)--(-552, -532)--(-558, -530), rgb(0.87, 0.19, 0.19)+linewidth(2)+solid); draw((-593, -588)--(-587, -593)--(-586, -599), rgb(0.87, 0.19, 0.19)+linewidth(2)+solid); draw((-520, -555)--(-530, -561), rgb(0.94, 0.54, 0)+linewidth(2)+solid); draw((-583, -557)--(-573, -563), rgb(0.94, 0.54, 0)+linewidth(2)+solid); label("$B$", (-500, -616.5), fontsize(20pt) + rgb(0.11, 0.11, 0.11)+linewidth(1)+solid); label("$A$", (-702, -618.5), fontsize(20pt) + rgb(0.11, 0.11, 0.11)+linewidth(1)+solid); label("$C$", (-702, -247.5), fontsize(20pt) + rgb(0.11, 0.11, 0.11)+linewidth(1)+solid); label("$1$", (-649, -623), fontsize(16pt) + rgb(0.11, 0.11, 0.11)+linewidth(1)+solid); label("$1$", (-555, -622), fontsize(16pt) + rgb(0.11, 0.11, 0.11)+linewidth(1)+solid); label("$1$", (-507, -548), fontsize(16pt) + rgb(0.11, 0.11, 0.11)+linewidth(1)+solid); label("$2\sqrt{3}$", (-732.5, -457), fontsize(16pt) + rgb(0.11, 0.11, 0.11)+linewidth(1)+solid); label("$3$", (-596, -385), fontsize(16pt) + rgb(0.11, 0.11, 0.11)+linewidth(1)+solid); label("$D$", (-635, -544.5), fontsize(20pt) + rgb(0.11, 0.11, 0.11)+linewidth(1)+solid); label("$M$", (-602, -620.5), fontsize(20pt) + rgb(0.11, 0.11, 0.11)+linewidth(1)+solid); label("$E$", (-534, -502.5), fontsize(20pt) + rgb(0.11, 0.11, 0.11)+linewidth(1)+solid); [/asy] WLOG $\overline{AB} = 2$ as the problem statement concerns only lengths ratios. Draw $\overline{EM}$ connecting the median of $\triangle ABE$ to right angle $\angle E$ , we know that by inscribing right $\triangle ABE$ in a circle and by Thales theorem, $\overline{ME} = \overline{MA} = \overline{MB}$ the circumradius. $\overline{MB} = \overline{ME} \iff \triangle BEM \text{ is isosceles}$ , and because $\angle B = 60^\circ$ , then $\angle E = 60^\circ$ , making $\triangle BEM$ equilateral.
Let $\overline{AD} = x$ and $\overline{DE} = y$ . By $30^\circ - 60^\circ - 90^\circ$ special right triangle \[\sqrt{3} = \overline{AE} = x + y\] \[\overline{AM} = \sqrt{(2\sqrt{3})^2 + 1^2} = \sqrt{13}\] \[\overline{CD} = \sqrt{y^2 + 3^2} = \sqrt{y^2 + 9} = \sqrt{x^2 - 2\sqrt{3}x + 12}\] \[\overline{DM} = \sqrt{x^2 + 1^2 - 2 \cdot 1 \cdot x \cdot \cos{30^\circ} } = \sqrt{x^2 - \sqrt{3}x + 1}\] \[\overline{CD} + \overline{DM} = \overline{AM}\] \[\sqrt{x^2 - 2\sqrt{3}x + 12} + \sqrt{x^2 - \sqrt{3}x + 1} = \sqrt{13}\] Algebra: \begin{align*} \sqrt{x^2 - 2\sqrt{3}x + 12} &= \sqrt{13} - \sqrt{x^2 - \sqrt{3}x + 1}\\ x^2 - 2\sqrt{3}x + 12 &= x^2 - \sqrt{3}x + 1 + 13 - 2\sqrt{13(x^2 - \sqrt{3}x + 1)}\\ -\sqrt{3}x - 2 &= -2\sqrt{13(x^2 - \sqrt{3}x + 1)}\\ 3x^2 + 4\sqrt{3}x + 4 &= 4\cdot13(x^2 - \sqrt{3}x + 1)\\ 49x^2 - 56\sqrt{3}x + 48 &= 0\\ (7x-4\sqrt{3})^2 &= 0 \end{align*} $x = \frac{4\sqrt{3}}{7}$ $y = \frac{3\sqrt{3}}{7}$ $x$ is defined to be minimum of those lengths, so $x = \frac{3\sqrt{3}}{7}$ Hence $\frac{x}{x+y} = \boxed{\frac{3}{7}}$
~clod

## Video Solution 1 by SpreadTheMathLove
https://www.youtube.com/watch?v=dLSWVrrKsgs

## Video Solution 2 (Fast and Easy)
https://www.youtube.com/watch?v=YhagQhoCM3A
~ Pi Academy
### See Also
These problems are copyrighted © by the Mathematical Association of America.
These problems are copyrighted © by the Mathematical Association of America.
These problems are copyrighted © by the Mathematical Association of America.
These problems are copyrighted © by the Mathematical Association of America .